Updating ERC20.bpl

benchmarks/openZeppelin/ERC20.bpl
@@ -1,14 +1,22 @@
+// #LTLProperty: [](started(ERC20.totalSupply) ==> <>(finished(ERC20.totalSupply, __ret_0_ == this._totalSupply && this._totalSupply == old(this._totalSupply) && this._balances == old(this._balances) && this._allowances == old(this._allowances))))
+// LTLProperty: [](started(ERC20.totalSupply) ==> <>(finished(ERC20.totalSupply, __ret_0_ == this._totalSupply && this._totalSupply == old(this._totalSupply) && M_Ref_int__balances0[_balances_ERC20[this]] == old(M_Ref_int__balances0[_balances_ERC20[this]]) && M_Ref_int__allowances1 == old(M_Ref_int__allowances1) && M_Ref_Ref__allowances1 == old(M_Ref_Ref__allowances1))))
 
-// #LTLProperty: [](started(ERC20.totalSupply) ==> <>(finished(ERC20.totalSupply, __ret_0_ == ERC20._totalSupply && ERC20._totalSupply == old(ERC20._totalSupply) && ERC20._balances == old(ERC20._balances) && ERC20._allowances == old(ERC20._allowances))))
+// LTLProperty: [](started(ERC20.balanceOf) ==> <>(finished(ERC20.balanceOf(owner), __ret_0_ == this._balances[owner] && this._totalSupply == old(this._totalSupply) && M_Ref_int__balances0[_balances_ERC20[this]] == old(M_Ref_int__balances0[_balances_ERC20[this]]) && M_Ref_int__allowances1 == old(M_Ref_int__allowances1) && M_Ref_Ref__allowances1 == old(M_Ref_Ref__allowances1))))
 
-type Ref;
-type ContractName;
+// LTLProperty: [](started(ERC20.allowance) ==> <>(finished(ERC20.allowance(owner, spender), __ret_0_ == this._allowances[owner][spender] && this._totalSupply == old(this._totalSupply) && M_Ref_int__balances0[_balances_ERC20[this]] == old(M_Ref_int__balances0[_balances_ERC20[this]]) && M_Ref_int__allowances1 == old(M_Ref_int__allowances1) && M_Ref_Ref__allowances1 == old(M_Ref_Ref__allowances1))))
+
+// LTLVariables: i0:Ref
+// LTLProperty: [](started(ERC20.allowance) ==> <>(finished(ERC20.allowance(owner, spender), __ret_0_ == this._allowances[owner][spender] && this._totalSupply == old(this._totalSupply) && M_Ref_int__balances0[_balances_ERC20[this]] == old(M_Ref_int__balances0[_balances_ERC20[this]]) && M_Ref_int__allowances1[M_Ref_Ref__allowances1[_allowances_ERC20[this]][i0]] == old(M_Ref_int__allowances1[M_Ref_Ref__allowances1[_allowances_ERC20[this]][i0]]))))
+
+type Ref = int;
+type ContractName = int;
 const unique null: Ref;
 const unique Context: ContractName;
 const unique SafeMath: ContractName;
 const unique IERC20: ContractName;
 const unique ERC20: ContractName;
-function ConstantToRef(x: int) returns (ret: Ref);
+function {:smtdefined "x"} ConstantToRef(x: int) returns (ret: Ref);
+function BoogieRefToInt(x: Ref) returns (ret: int);
 function {:bvbuiltin "mod"} modBpl(x: int, y: int) returns (ret: int);
 function keccak256(x: int) returns (ret: int);
 function abiEncodePacked1(x: int) returns (ret: int);
@@ -22,30 +30,44 @@ function {:smtdefined "((as const (Array Int Bool)) false)"} zeroRefBoolArr() re
 function {:smtdefined "((as const (Array Int Bool)) false)"} zeroIntBoolArr() returns (ret: [int]bool);
 function {:smtdefined "((as const (Array Int Int)) 0)"} zeroRefRefArr() returns (ret: [Ref]Ref);
 function {:smtdefined "((as const (Array Int Int)) 0)"} zeroIntRefArr() returns (ret: [int]Ref);
+function nonlinearMul(x: int, y: int) returns (ret: int);
+function nonlinearDiv(x: int, y: int) returns (ret: int);
+function nonlinearPow(x: int, y: int) returns (ret: int);
+function nonlinearMod(x: int, y: int) returns (ret: int);
 var Balance: [Ref]int;
 var DType: [Ref]ContractName;
 var Alloc: [Ref]bool;
 var balance_ADDR: [Ref]int;
-var M_Ref_int: [Ref][Ref]int;
-var M_Ref_Ref: [Ref][Ref]Ref;
+var M_Ref_int__balances0: [Ref][Ref]int;
+var sum__balances0: [Ref]int;
+var M_Ref_int__allowances1: [Ref][Ref]int;
+var M_Ref_Ref__allowances1: [Ref][Ref]Ref;
+var sum__allowances1: [Ref]int;
 var Length: [Ref]int;
 var revert: bool;
 var gas: int;
+var now: int;
 procedure {:inline 1} FreshRefGenerator__success() returns (newRef: Ref);
 modifies Alloc;
 procedure {:inline 1} Context_Context_NoBaseCtor__success(this: Ref, msgsender_MSG: Ref, msgvalue_MSG: int);
+modifies Balance;
 procedure {:constructor} {:public} {:inline 1} Context_Context(this: Ref, msgsender_MSG: Ref, msgvalue_MSG: int);
 modifies revert;
 modifies __tmp__Balance;
 modifies __tmp__DType;
 modifies __tmp__Alloc;
 modifies __tmp__balance_ADDR;
-modifies __tmp__M_Ref_int;
-modifies __tmp__M_Ref_Ref;
+modifies __tmp__M_Ref_int__balances0;
+modifies __tmp__sum__balances0;
+modifies __tmp__M_Ref_int__allowances1;
+modifies __tmp__M_Ref_Ref__allowances1;
+modifies __tmp__sum__allowances1;
 modifies __tmp__Length;
+modifies __tmp__now;
 modifies __tmp___balances_ERC20;
 modifies __tmp___allowances_ERC20;
 modifies __tmp___totalSupply_ERC20;
+modifies Balance;
 implementation Context_Context(this: Ref, msgsender_MSG: Ref, msgvalue_MSG: int)
 {
 var __exception: bool;
@@ -56,9 +78,13 @@ __tmp__Balance := Balance;
 __tmp__DType := DType;
 __tmp__Alloc := Alloc;
 __tmp__balance_ADDR := balance_ADDR;
-__tmp__M_Ref_int := M_Ref_int;
-__tmp__M_Ref_Ref := M_Ref_Ref;
+__tmp__M_Ref_int__balances0 := M_Ref_int__balances0;
+__tmp__sum__balances0 := sum__balances0;
+__tmp__M_Ref_int__allowances1 := M_Ref_int__allowances1;
+__tmp__M_Ref_Ref__allowances1 := M_Ref_Ref__allowances1;
+__tmp__sum__allowances1 := sum__allowances1;
 __tmp__Length := Length;
+__tmp__now := now;
 __tmp___balances_ERC20 := _balances_ERC20;
 __tmp___allowances_ERC20 := _allowances_ERC20;
 __tmp___totalSupply_ERC20 := _totalSupply_ERC20;
@@ -71,19 +97,26 @@ assume ((!(revert)) && ((gas) >= (0)));
 }
 
 procedure {:inline 1} _msgSender_Context__success(this: Ref, msgsender_MSG: Ref, msgvalue_MSG: int) returns (__ret_0_: Ref);
+modifies gas;
 procedure {:inline 1} SafeMath_SafeMath_NoBaseCtor__success(this: Ref, msgsender_MSG: Ref, msgvalue_MSG: int);
+modifies Balance;
 procedure {:inline 1} SafeMath_SafeMath(this: Ref, msgsender_MSG: Ref, msgvalue_MSG: int);
 modifies revert;
 modifies __tmp__Balance;
 modifies __tmp__DType;
 modifies __tmp__Alloc;
 modifies __tmp__balance_ADDR;
-modifies __tmp__M_Ref_int;
-modifies __tmp__M_Ref_Ref;
+modifies __tmp__M_Ref_int__balances0;
+modifies __tmp__sum__balances0;
+modifies __tmp__M_Ref_int__allowances1;
+modifies __tmp__M_Ref_Ref__allowances1;
+modifies __tmp__sum__allowances1;
 modifies __tmp__Length;
+modifies __tmp__now;
 modifies __tmp___balances_ERC20;
 modifies __tmp___allowances_ERC20;
 modifies __tmp___totalSupply_ERC20;
+modifies Balance;
 implementation SafeMath_SafeMath(this: Ref, msgsender_MSG: Ref, msgvalue_MSG: int)
 {
 var __exception: bool;
@@ -94,9 +127,13 @@ __tmp__Balance := Balance;
 __tmp__DType := DType;
 __tmp__Alloc := Alloc;
 __tmp__balance_ADDR := balance_ADDR;
-__tmp__M_Ref_int := M_Ref_int;
-__tmp__M_Ref_Ref := M_Ref_Ref;
+__tmp__M_Ref_int__balances0 := M_Ref_int__balances0;
+__tmp__sum__balances0 := sum__balances0;
+__tmp__M_Ref_int__allowances1 := M_Ref_int__allowances1;
+__tmp__M_Ref_Ref__allowances1 := M_Ref_Ref__allowances1;
+__tmp__sum__allowances1 := sum__allowances1;
 __tmp__Length := Length;
+__tmp__now := now;
 __tmp___balances_ERC20 := _balances_ERC20;
 __tmp___allowances_ERC20 := _allowances_ERC20;
 __tmp___totalSupply_ERC20 := _totalSupply_ERC20;
@@ -109,8 +146,10 @@ assume ((!(revert)) && ((gas) >= (0)));
 }
 
 procedure {:inline 1} add_SafeMath__success(this: Ref, msgsender_MSG: Ref, msgvalue_MSG: int, a_s40: int, b_s40: int) returns (__ret_0_: int);
+modifies gas;
 modifies revert;
 procedure {:inline 1} sub_SafeMath__success(this: Ref, msgsender_MSG: Ref, msgvalue_MSG: int, a_s65: int, b_s65: int) returns (__ret_0_: int);
+modifies gas;
 modifies revert;
 procedure {:inline 1} mul_SafeMath__success(this: Ref, msgsender_MSG: Ref, msgvalue_MSG: int, a_s99: int, b_s99: int) returns (__ret_0_: int);
 modifies revert;
@@ -119,18 +158,24 @@ modifies revert;
 procedure {:inline 1} mod_SafeMath__success(this: Ref, msgsender_MSG: Ref, msgvalue_MSG: int, a_s145: int, b_s145: int) returns (__ret_0_: int);
 modifies revert;
 procedure {:inline 1} IERC20_IERC20_NoBaseCtor__success(this: Ref, msgsender_MSG: Ref, msgvalue_MSG: int);
+modifies Balance;
 procedure {:inline 1} IERC20_IERC20(this: Ref, msgsender_MSG: Ref, msgvalue_MSG: int);
 modifies revert;
 modifies __tmp__Balance;
 modifies __tmp__DType;
 modifies __tmp__Alloc;
 modifies __tmp__balance_ADDR;
-modifies __tmp__M_Ref_int;
-modifies __tmp__M_Ref_Ref;
+modifies __tmp__M_Ref_int__balances0;
+modifies __tmp__sum__balances0;
+modifies __tmp__M_Ref_int__allowances1;
+modifies __tmp__M_Ref_Ref__allowances1;
+modifies __tmp__sum__allowances1;
 modifies __tmp__Length;
+modifies __tmp__now;
 modifies __tmp___balances_ERC20;
 modifies __tmp___allowances_ERC20;
 modifies __tmp___totalSupply_ERC20;
+modifies Balance;
 implementation IERC20_IERC20(this: Ref, msgsender_MSG: Ref, msgvalue_MSG: int)
 {
 var __exception: bool;
@@ -141,9 +186,13 @@ __tmp__Balance := Balance;
 __tmp__DType := DType;
 __tmp__Alloc := Alloc;
 __tmp__balance_ADDR := balance_ADDR;
-__tmp__M_Ref_int := M_Ref_int;
-__tmp__M_Ref_Ref := M_Ref_Ref;
+__tmp__M_Ref_int__balances0 := M_Ref_int__balances0;
+__tmp__sum__balances0 := sum__balances0;
+__tmp__M_Ref_int__allowances1 := M_Ref_int__allowances1;
+__tmp__M_Ref_Ref__allowances1 := M_Ref_Ref__allowances1;
+__tmp__sum__allowances1 := sum__allowances1;
 __tmp__Length := Length;
+__tmp__now := now;
 __tmp___balances_ERC20 := _balances_ERC20;
 __tmp___allowances_ERC20 := _allowances_ERC20;
 __tmp___totalSupply_ERC20 := _totalSupply_ERC20;
@@ -162,11 +211,14 @@ procedure {:public} {:inline 1} allowance_IERC20(this: Ref, msgsender_MSG: Ref, 
 procedure {:public} {:inline 1} approve_IERC20(this: Ref, msgsender_MSG: Ref, msgvalue_MSG: int, spender_s185: Ref, amount_s185: int) returns (__ret_0_: bool);
 procedure {:public} {:inline 1} transferFrom_IERC20(this: Ref, msgsender_MSG: Ref, msgvalue_MSG: int, sender_s196: Ref, recipient_s196: Ref, amount_s196: int) returns (__ret_0_: bool);
 procedure {:inline 1} ERC20_ERC20_NoBaseCtor__success(this: Ref, msgsender_MSG: Ref, msgvalue_MSG: int);
-modifies _totalSupply_ERC20;
+modifies Balance;
 modifies _balances_ERC20;
-modifies M_Ref_int;
+modifies M_Ref_int__balances0;
+modifies sum__balances0;
 modifies _allowances_ERC20;
-modifies M_Ref_Ref;
+modifies M_Ref_Ref__allowances1;
+modifies M_Ref_int__allowances1;
+modifies _totalSupply_ERC20;
 modifies Alloc;
 procedure {:inline 1} ERC20_ERC20(this: Ref, msgsender_MSG: Ref, msgvalue_MSG: int);
 modifies revert;
@@ -174,17 +226,24 @@ modifies __tmp__Balance;
 modifies __tmp__DType;
 modifies __tmp__Alloc;
 modifies __tmp__balance_ADDR;
-modifies __tmp__M_Ref_int;
-modifies __tmp__M_Ref_Ref;
+modifies __tmp__M_Ref_int__balances0;
+modifies __tmp__sum__balances0;
+modifies __tmp__M_Ref_int__allowances1;
+modifies __tmp__M_Ref_Ref__allowances1;
+modifies __tmp__sum__allowances1;
 modifies __tmp__Length;
+modifies __tmp__now;
 modifies __tmp___balances_ERC20;
 modifies __tmp___allowances_ERC20;
 modifies __tmp___totalSupply_ERC20;
-modifies _totalSupply_ERC20;
+modifies Balance;
 modifies _balances_ERC20;
-modifies M_Ref_int;
+modifies M_Ref_int__balances0;
+modifies sum__balances0;
 modifies _allowances_ERC20;
-modifies M_Ref_Ref;
+modifies M_Ref_Ref__allowances1;
+modifies M_Ref_int__allowances1;
+modifies _totalSupply_ERC20;
 modifies Alloc;
 implementation ERC20_ERC20(this: Ref, msgsender_MSG: Ref, msgvalue_MSG: int)
 {
@@ -196,9 +255,13 @@ __tmp__Balance := Balance;
 __tmp__DType := DType;
 __tmp__Alloc := Alloc;
 __tmp__balance_ADDR := balance_ADDR;
-__tmp__M_Ref_int := M_Ref_int;
-__tmp__M_Ref_Ref := M_Ref_Ref;
+__tmp__M_Ref_int__balances0 := M_Ref_int__balances0;
+__tmp__sum__balances0 := sum__balances0;
+__tmp__M_Ref_int__allowances1 := M_Ref_int__allowances1;
+__tmp__M_Ref_Ref__allowances1 := M_Ref_Ref__allowances1;
+__tmp__sum__allowances1 := sum__allowances1;
 __tmp__Length := Length;
+__tmp__now := now;
 __tmp___balances_ERC20 := _balances_ERC20;
 __tmp___allowances_ERC20 := _allowances_ERC20;
 __tmp___totalSupply_ERC20 := _totalSupply_ERC20;
@@ -210,21 +273,26 @@ assume ((!(revert)) && ((gas) >= (0)));
 }
 }
 
-var _balances_ERC20: [Ref]Ref;
-var _allowances_ERC20: [Ref]Ref;
-var _totalSupply_ERC20: [Ref]int;
+var {:access "this._balances[i0]=M_Ref_int__balances0[_balances_ERC20[this]][i0]"} {:sum "sum(this._balances)=sum__balances0[_balances_ERC20[this]]"} _balances_ERC20: [Ref]Ref;
+var {:access "this._allowances[i0][i1]=M_Ref_int__allowances1[M_Ref_Ref__allowances1[_allowances_ERC20[this]][i0]][i1]"} {:sum "sum(this._allowances)=sum__allowances1[_allowances_ERC20[this]]"} _allowances_ERC20: [Ref]Ref;
+var {:access "this._totalSupply=_totalSupply_ERC20[this]"} _totalSupply_ERC20: [Ref]int;
 procedure {:public} {:inline 1} totalSupply_ERC20(this: Ref, msgsender_MSG: Ref, msgvalue_MSG: int) returns (__ret_0_: int);
 modifies revert;
 modifies __tmp__Balance;
 modifies __tmp__DType;
 modifies __tmp__Alloc;
 modifies __tmp__balance_ADDR;
-modifies __tmp__M_Ref_int;
-modifies __tmp__M_Ref_Ref;
+modifies __tmp__M_Ref_int__balances0;
+modifies __tmp__sum__balances0;
+modifies __tmp__M_Ref_int__allowances1;
+modifies __tmp__M_Ref_Ref__allowances1;
+modifies __tmp__sum__allowances1;
 modifies __tmp__Length;
+modifies __tmp__now;
 modifies __tmp___balances_ERC20;
 modifies __tmp___allowances_ERC20;
 modifies __tmp___totalSupply_ERC20;
+modifies gas;
 implementation totalSupply_ERC20(this: Ref, msgsender_MSG: Ref, msgvalue_MSG: int) returns (__ret_0_: int)
 {
 var __exception: bool;
@@ -235,9 +303,13 @@ __tmp__Balance := Balance;
 __tmp__DType := DType;
 __tmp__Alloc := Alloc;
 __tmp__balance_ADDR := balance_ADDR;
-__tmp__M_Ref_int := M_Ref_int;
-__tmp__M_Ref_Ref := M_Ref_Ref;
+__tmp__M_Ref_int__balances0 := M_Ref_int__balances0;
+__tmp__sum__balances0 := sum__balances0;
+__tmp__M_Ref_int__allowances1 := M_Ref_int__allowances1;
+__tmp__M_Ref_Ref__allowances1 := M_Ref_Ref__allowances1;
+__tmp__sum__allowances1 := sum__allowances1;
 __tmp__Length := Length;
+__tmp__now := now;
 __tmp___balances_ERC20 := _balances_ERC20;
 __tmp___allowances_ERC20 := _allowances_ERC20;
 __tmp___totalSupply_ERC20 := _totalSupply_ERC20;
@@ -255,12 +327,17 @@ modifies __tmp__Balance;
 modifies __tmp__DType;
 modifies __tmp__Alloc;
 modifies __tmp__balance_ADDR;
-modifies __tmp__M_Ref_int;
-modifies __tmp__M_Ref_Ref;
+modifies __tmp__M_Ref_int__balances0;
+modifies __tmp__sum__balances0;
+modifies __tmp__M_Ref_int__allowances1;
+modifies __tmp__M_Ref_Ref__allowances1;
+modifies __tmp__sum__allowances1;
 modifies __tmp__Length;
+modifies __tmp__now;
 modifies __tmp___balances_ERC20;
 modifies __tmp___allowances_ERC20;
 modifies __tmp___totalSupply_ERC20;
+modifies gas;
 implementation balanceOf_ERC20(this: Ref, msgsender_MSG: Ref, msgvalue_MSG: int, account_s252: Ref) returns (__ret_0_: int)
 {
 var __exception: bool;
@@ -271,9 +348,13 @@ __tmp__Balance := Balance;
 __tmp__DType := DType;
 __tmp__Alloc := Alloc;
 __tmp__balance_ADDR := balance_ADDR;
-__tmp__M_Ref_int := M_Ref_int;
-__tmp__M_Ref_Ref := M_Ref_Ref;
+__tmp__M_Ref_int__balances0 := M_Ref_int__balances0;
+__tmp__sum__balances0 := sum__balances0;
+__tmp__M_Ref_int__allowances1 := M_Ref_int__allowances1;
+__tmp__M_Ref_Ref__allowances1 := M_Ref_Ref__allowances1;
+__tmp__sum__allowances1 := sum__allowances1;
 __tmp__Length := Length;
+__tmp__now := now;
 __tmp___balances_ERC20 := _balances_ERC20;
 __tmp___allowances_ERC20 := _allowances_ERC20;
 __tmp___totalSupply_ERC20 := _totalSupply_ERC20;
@@ -291,13 +372,19 @@ modifies __tmp__Balance;
 modifies __tmp__DType;
 modifies __tmp__Alloc;
 modifies __tmp__balance_ADDR;
-modifies __tmp__M_Ref_int;
-modifies __tmp__M_Ref_Ref;
+modifies __tmp__M_Ref_int__balances0;
+modifies __tmp__sum__balances0;
+modifies __tmp__M_Ref_int__allowances1;
+modifies __tmp__M_Ref_Ref__allowances1;
+modifies __tmp__sum__allowances1;
 modifies __tmp__Length;
+modifies __tmp__now;
 modifies __tmp___balances_ERC20;
 modifies __tmp___allowances_ERC20;
 modifies __tmp___totalSupply_ERC20;
-modifies M_Ref_int;
+modifies gas;
+modifies sum__balances0;
+modifies M_Ref_int__balances0;
 implementation transfer_ERC20(this: Ref, msgsender_MSG: Ref, msgvalue_MSG: int, recipient_s267: Ref, amount_s267: int) returns (__ret_0_: bool)
 {
 var __exception: bool;
@@ -308,9 +395,13 @@ __tmp__Balance := Balance;
 __tmp__DType := DType;
 __tmp__Alloc := Alloc;
 __tmp__balance_ADDR := balance_ADDR;
-__tmp__M_Ref_int := M_Ref_int;
-__tmp__M_Ref_Ref := M_Ref_Ref;
+__tmp__M_Ref_int__balances0 := M_Ref_int__balances0;
+__tmp__sum__balances0 := sum__balances0;
+__tmp__M_Ref_int__allowances1 := M_Ref_int__allowances1;
+__tmp__M_Ref_Ref__allowances1 := M_Ref_Ref__allowances1;
+__tmp__sum__allowances1 := sum__allowances1;
 __tmp__Length := Length;
+__tmp__now := now;
 __tmp___balances_ERC20 := _balances_ERC20;
 __tmp___allowances_ERC20 := _allowances_ERC20;
 __tmp___totalSupply_ERC20 := _totalSupply_ERC20;
@@ -323,22 +414,30 @@ assume ((!(revert)) && ((gas) >= (0)));
 }
 
 procedure {:inline 1} transfer_ERC20_ERC20__success(this: Ref, msgsender_MSG: Ref, msgvalue_MSG: int, recipient_s286: Ref, amount_s286: int) returns (__ret_0_: bool);
+modifies gas;
 modifies revert;
-modifies M_Ref_int;
+modifies sum__balances0;
+modifies M_Ref_int__balances0;
 procedure {:public} {:inline 1} allowance_ERC20(this: Ref, msgsender_MSG: Ref, msgvalue_MSG: int, owner_s302: Ref, spender_s302: Ref) returns (__ret_0_: int);
 modifies revert;
 modifies __tmp__Balance;
 modifies __tmp__DType;
 modifies __tmp__Alloc;
 modifies __tmp__balance_ADDR;
-modifies __tmp__M_Ref_int;
-modifies __tmp__M_Ref_Ref;
+modifies __tmp__M_Ref_int__balances0;
+modifies __tmp__sum__balances0;
+modifies __tmp__M_Ref_int__allowances1;
+modifies __tmp__M_Ref_Ref__allowances1;
+modifies __tmp__sum__allowances1;
 modifies __tmp__Length;
+modifies __tmp__now;
 modifies __tmp___balances_ERC20;
 modifies __tmp___allowances_ERC20;
 modifies __tmp___totalSupply_ERC20;
-modifies M_Ref_Ref;
-modifies M_Ref_int;
+modifies gas;
+modifies M_Ref_Ref__allowances1;
+modifies M_Ref_int__allowances1;
+modifies sum__allowances1;
 modifies Alloc;
 implementation allowance_ERC20(this: Ref, msgsender_MSG: Ref, msgvalue_MSG: int, owner_s302: Ref, spender_s302: Ref) returns (__ret_0_: int)
 {
@@ -350,9 +449,13 @@ __tmp__Balance := Balance;
 __tmp__DType := DType;
 __tmp__Alloc := Alloc;
 __tmp__balance_ADDR := balance_ADDR;
-__tmp__M_Ref_int := M_Ref_int;
-__tmp__M_Ref_Ref := M_Ref_Ref;
+__tmp__M_Ref_int__balances0 := M_Ref_int__balances0;
+__tmp__sum__balances0 := sum__balances0;
+__tmp__M_Ref_int__allowances1 := M_Ref_int__allowances1;
+__tmp__M_Ref_Ref__allowances1 := M_Ref_Ref__allowances1;
+__tmp__sum__allowances1 := sum__allowances1;
 __tmp__Length := Length;
+__tmp__now := now;
 __tmp___balances_ERC20 := _balances_ERC20;
 __tmp___allowances_ERC20 := _allowances_ERC20;
 __tmp___totalSupply_ERC20 := _totalSupply_ERC20;
@@ -370,14 +473,20 @@ modifies __tmp__Balance;
 modifies __tmp__DType;
 modifies __tmp__Alloc;
 modifies __tmp__balance_ADDR;
-modifies __tmp__M_Ref_int;
-modifies __tmp__M_Ref_Ref;
+modifies __tmp__M_Ref_int__balances0;
+modifies __tmp__sum__balances0;
+modifies __tmp__M_Ref_int__allowances1;
+modifies __tmp__M_Ref_Ref__allowances1;
+modifies __tmp__sum__allowances1;
 modifies __tmp__Length;
+modifies __tmp__now;
 modifies __tmp___balances_ERC20;
 modifies __tmp___allowances_ERC20;
 modifies __tmp___totalSupply_ERC20;
-modifies M_Ref_Ref;
-modifies M_Ref_int;
+modifies gas;
+modifies M_Ref_Ref__allowances1;
+modifies M_Ref_int__allowances1;
+modifies sum__allowances1;
 modifies Alloc;
 implementation approve_ERC20(this: Ref, msgsender_MSG: Ref, msgvalue_MSG: int, spender_s317: Ref, amount_s317: int) returns (__ret_0_: bool)
 {
@@ -389,9 +498,13 @@ __tmp__Balance := Balance;
 __tmp__DType := DType;
 __tmp__Alloc := Alloc;
 __tmp__balance_ADDR := balance_ADDR;
-__tmp__M_Ref_int := M_Ref_int;
-__tmp__M_Ref_Ref := M_Ref_Ref;
+__tmp__M_Ref_int__balances0 := M_Ref_int__balances0;
+__tmp__sum__balances0 := sum__balances0;
+__tmp__M_Ref_int__allowances1 := M_Ref_int__allowances1;
+__tmp__M_Ref_Ref__allowances1 := M_Ref_Ref__allowances1;
+__tmp__sum__allowances1 := sum__allowances1;
 __tmp__Length := Length;
+__tmp__now := now;
 __tmp___balances_ERC20 := _balances_ERC20;
 __tmp___allowances_ERC20 := _allowances_ERC20;
 __tmp___totalSupply_ERC20 := _totalSupply_ERC20;
@@ -404,9 +517,11 @@ assume ((!(revert)) && ((gas) >= (0)));
 }
 
 procedure {:inline 1} approve_ERC20_ERC20__success(this: Ref, msgsender_MSG: Ref, msgvalue_MSG: int, spender_s336: Ref, amount_s336: int) returns (__ret_0_: bool);
+modifies gas;
 modifies revert;
-modifies M_Ref_Ref;
-modifies M_Ref_int;
+modifies M_Ref_Ref__allowances1;
+modifies M_Ref_int__allowances1;
+modifies sum__allowances1;
 modifies Alloc;
 procedure {:public} {:inline 1} transferFrom_ERC20(this: Ref, msgsender_MSG: Ref, msgvalue_MSG: int, sender_s354: Ref, recipient_s354: Ref, amount_s354: int) returns (__ret_0_: bool);
 modifies revert;
@@ -414,14 +529,22 @@ modifies __tmp__Balance;
 modifies __tmp__DType;
 modifies __tmp__Alloc;
 modifies __tmp__balance_ADDR;
-modifies __tmp__M_Ref_int;
-modifies __tmp__M_Ref_Ref;
+modifies __tmp__M_Ref_int__balances0;
+modifies __tmp__sum__balances0;
+modifies __tmp__M_Ref_int__allowances1;
+modifies __tmp__M_Ref_Ref__allowances1;
+modifies __tmp__sum__allowances1;
 modifies __tmp__Length;
+modifies __tmp__now;
 modifies __tmp___balances_ERC20;
 modifies __tmp___allowances_ERC20;
 modifies __tmp___totalSupply_ERC20;
-modifies M_Ref_Ref;
-modifies M_Ref_int;
+modifies gas;
+modifies M_Ref_Ref__allowances1;
+modifies M_Ref_int__allowances1;
+modifies sum__allowances1;
+modifies sum__balances0;
+modifies M_Ref_int__balances0;
 modifies Alloc;
 implementation transferFrom_ERC20(this: Ref, msgsender_MSG: Ref, msgvalue_MSG: int, sender_s354: Ref, recipient_s354: Ref, amount_s354: int) returns (__ret_0_: bool)
 {
@@ -433,9 +556,13 @@ __tmp__Balance := Balance;
 __tmp__DType := DType;
 __tmp__Alloc := Alloc;
 __tmp__balance_ADDR := balance_ADDR;
-__tmp__M_Ref_int := M_Ref_int;
-__tmp__M_Ref_Ref := M_Ref_Ref;
+__tmp__M_Ref_int__balances0 := M_Ref_int__balances0;
+__tmp__sum__balances0 := sum__balances0;
+__tmp__M_Ref_int__allowances1 := M_Ref_int__allowances1;
+__tmp__M_Ref_Ref__allowances1 := M_Ref_Ref__allowances1;
+__tmp__sum__allowances1 := sum__allowances1;
 __tmp__Length := Length;
+__tmp__now := now;
 __tmp___balances_ERC20 := _balances_ERC20;
 __tmp___allowances_ERC20 := _allowances_ERC20;
 __tmp___totalSupply_ERC20 := _totalSupply_ERC20;
@@ -448,9 +575,13 @@ assume ((!(revert)) && ((gas) >= (0)));
 }
 
 procedure {:inline 1} transferFrom_ERC20_ERC20__success(this: Ref, msgsender_MSG: Ref, msgvalue_MSG: int, sender_s389: Ref, recipient_s389: Ref, amount_s389: int) returns (__ret_0_: bool);
-modifies M_Ref_Ref;
-modifies M_Ref_int;
+modifies gas;
+modifies M_Ref_Ref__allowances1;
+modifies M_Ref_int__allowances1;
+modifies sum__allowances1;
 modifies revert;
+modifies sum__balances0;
+modifies M_Ref_int__balances0;
 modifies Alloc;
 procedure {:public} {:inline 1} increaseAllowance_ERC20(this: Ref, msgsender_MSG: Ref, msgvalue_MSG: int, spender_s404: Ref, addedValue_s404: int) returns (__ret_0_: bool);
 modifies revert;
@@ -458,14 +589,20 @@ modifies __tmp__Balance;
 modifies __tmp__DType;
 modifies __tmp__Alloc;
 modifies __tmp__balance_ADDR;
-modifies __tmp__M_Ref_int;
-modifies __tmp__M_Ref_Ref;
+modifies __tmp__M_Ref_int__balances0;
+modifies __tmp__sum__balances0;
+modifies __tmp__M_Ref_int__allowances1;
+modifies __tmp__M_Ref_Ref__allowances1;
+modifies __tmp__sum__allowances1;
 modifies __tmp__Length;
+modifies __tmp__now;
 modifies __tmp___balances_ERC20;
 modifies __tmp___allowances_ERC20;
 modifies __tmp___totalSupply_ERC20;
-modifies M_Ref_Ref;
-modifies M_Ref_int;
+modifies gas;
+modifies M_Ref_Ref__allowances1;
+modifies M_Ref_int__allowances1;
+modifies sum__allowances1;
 modifies Alloc;
 implementation increaseAllowance_ERC20(this: Ref, msgsender_MSG: Ref, msgvalue_MSG: int, spender_s404: Ref, addedValue_s404: int) returns (__ret_0_: bool)
 {
@@ -477,9 +614,13 @@ __tmp__Balance := Balance;
 __tmp__DType := DType;
 __tmp__Alloc := Alloc;
 __tmp__balance_ADDR := balance_ADDR;
-__tmp__M_Ref_int := M_Ref_int;
-__tmp__M_Ref_Ref := M_Ref_Ref;
+__tmp__M_Ref_int__balances0 := M_Ref_int__balances0;
+__tmp__sum__balances0 := sum__balances0;
+__tmp__M_Ref_int__allowances1 := M_Ref_int__allowances1;
+__tmp__M_Ref_Ref__allowances1 := M_Ref_Ref__allowances1;
+__tmp__sum__allowances1 := sum__allowances1;
 __tmp__Length := Length;
+__tmp__now := now;
 __tmp___balances_ERC20 := _balances_ERC20;
 __tmp___allowances_ERC20 := _allowances_ERC20;
 __tmp___totalSupply_ERC20 := _totalSupply_ERC20;
@@ -492,8 +633,10 @@ assume ((!(revert)) && ((gas) >= (0)));
 }
 
 procedure {:inline 1} increaseAllowance_ERC20_ERC20__success(this: Ref, msgsender_MSG: Ref, msgvalue_MSG: int, spender_s431: Ref, addedValue_s431: int) returns (__ret_0_: bool);
-modifies M_Ref_Ref;
-modifies M_Ref_int;
+modifies gas;
+modifies M_Ref_Ref__allowances1;
+modifies M_Ref_int__allowances1;
+modifies sum__allowances1;
 modifies Alloc;
 modifies revert;
 procedure {:public} {:inline 1} decreaseAllowance_ERC20(this: Ref, msgsender_MSG: Ref, msgvalue_MSG: int, spender_s446: Ref, subtractedValue_s446: int) returns (__ret_0_: bool);
@@ -502,14 +645,20 @@ modifies __tmp__Balance;
 modifies __tmp__DType;
 modifies __tmp__Alloc;
 modifies __tmp__balance_ADDR;
-modifies __tmp__M_Ref_int;
-modifies __tmp__M_Ref_Ref;
+modifies __tmp__M_Ref_int__balances0;
+modifies __tmp__sum__balances0;
+modifies __tmp__M_Ref_int__allowances1;
+modifies __tmp__M_Ref_Ref__allowances1;
+modifies __tmp__sum__allowances1;
 modifies __tmp__Length;
+modifies __tmp__now;
 modifies __tmp___balances_ERC20;
 modifies __tmp___allowances_ERC20;
 modifies __tmp___totalSupply_ERC20;
-modifies M_Ref_Ref;
-modifies M_Ref_int;
+modifies gas;
+modifies M_Ref_Ref__allowances1;
+modifies M_Ref_int__allowances1;
+modifies sum__allowances1;
 modifies Alloc;
 implementation decreaseAllowance_ERC20(this: Ref, msgsender_MSG: Ref, msgvalue_MSG: int, spender_s446: Ref, subtractedValue_s446: int) returns (__ret_0_: bool)
 {
@@ -521,9 +670,13 @@ __tmp__Balance := Balance;
 __tmp__DType := DType;
 __tmp__Alloc := Alloc;
 __tmp__balance_ADDR := balance_ADDR;
-__tmp__M_Ref_int := M_Ref_int;
-__tmp__M_Ref_Ref := M_Ref_Ref;
+__tmp__M_Ref_int__balances0 := M_Ref_int__balances0;
+__tmp__sum__balances0 := sum__balances0;
+__tmp__M_Ref_int__allowances1 := M_Ref_int__allowances1;
+__tmp__M_Ref_Ref__allowances1 := M_Ref_Ref__allowances1;
+__tmp__sum__allowances1 := sum__allowances1;
 __tmp__Length := Length;
+__tmp__now := now;
 __tmp___balances_ERC20 := _balances_ERC20;
 __tmp___allowances_ERC20 := _allowances_ERC20;
 __tmp___totalSupply_ERC20 := _totalSupply_ERC20;
@@ -536,183 +689,225 @@ assume ((!(revert)) && ((gas) >= (0)));
 }
 
 procedure {:inline 1} decreaseAllowance_ERC20_ERC20__success(this: Ref, msgsender_MSG: Ref, msgvalue_MSG: int, spender_s473: Ref, subtractedValue_s473: int) returns (__ret_0_: bool);
-modifies M_Ref_Ref;
-modifies M_Ref_int;
+modifies gas;
+modifies M_Ref_Ref__allowances1;
+modifies M_Ref_int__allowances1;
+modifies sum__allowances1;
 modifies Alloc;
 modifies revert;
 procedure {:inline 1} _transfer_ERC20__success(this: Ref, msgsender_MSG: Ref, msgvalue_MSG: int, sender_s529: Ref, recipient_s529: Ref, amount_s529: int);
+modifies gas;
 modifies revert;
-modifies M_Ref_int;
+modifies sum__balances0;
+modifies M_Ref_int__balances0;
 procedure {:inline 1} _mint_ERC20__success(this: Ref, msgsender_MSG: Ref, msgvalue_MSG: int, account_s542: Ref, amount_s542: int);
 modifies revert;
 modifies _totalSupply_ERC20;
-modifies M_Ref_int;
+modifies sum__balances0;
+modifies M_Ref_int__balances0;
+modifies gas;
 procedure {:inline 1} _mint_ERC20_ERC20__success(this: Ref, msgsender_MSG: Ref, msgvalue_MSG: int, account_s585: Ref, amount_s585: int);
 modifies revert;
 modifies _totalSupply_ERC20;
-modifies M_Ref_int;
+modifies sum__balances0;
+modifies M_Ref_int__balances0;
+modifies gas;
 procedure {:inline 1} _burn_ERC20__success(this: Ref, msgsender_MSG: Ref, msgvalue_MSG: int, account_s628: Ref, amount_s628: int);
 modifies revert;
-modifies M_Ref_int;
+modifies sum__balances0;
+modifies M_Ref_int__balances0;
 modifies _totalSupply_ERC20;
+modifies gas;
 procedure {:inline 1} _approve_ERC20__success(this: Ref, msgsender_MSG: Ref, msgvalue_MSG: int, owner_s670: Ref, spender_s670: Ref, amount_s670: int);
+modifies gas;
 modifies revert;
-modifies M_Ref_Ref;
-modifies M_Ref_int;
+modifies M_Ref_Ref__allowances1;
+modifies M_Ref_int__allowances1;
+modifies sum__allowances1;
 modifies Alloc;
 procedure {:inline 1} _burnFrom_ERC20__success(this: Ref, msgsender_MSG: Ref, msgvalue_MSG: int, account_s698: Ref, amount_s698: int);
-modifies M_Ref_Ref;
-modifies M_Ref_int;
+modifies M_Ref_Ref__allowances1;
+modifies M_Ref_int__allowances1;
+modifies sum__allowances1;
 modifies revert;
+modifies sum__balances0;
+modifies M_Ref_int__balances0;
 modifies _totalSupply_ERC20;
+modifies gas;
 modifies Alloc;
 procedure {:inline 1} FallbackDispatch__success(from: Ref, to: Ref, amount: int);
 modifies Balance;
-modifies gas;
-modifies M_Ref_Ref;
-modifies M_Ref_int;
-modifies Alloc;
 modifies revert;
+modifies gas;
+modifies M_Ref_Ref__allowances1;
+modifies M_Ref_int__allowances1;
+modifies sum__allowances1;
+modifies Alloc;
+modifies sum__balances0;
+modifies M_Ref_int__balances0;
 procedure {:inline 1} Fallback_UnknownType__success(from: Ref, to: Ref, amount: int);
 modifies Balance;
-modifies gas;
-modifies M_Ref_Ref;
-modifies M_Ref_int;
-modifies Alloc;
 modifies revert;
+modifies gas;
+modifies M_Ref_Ref__allowances1;
+modifies M_Ref_int__allowances1;
+modifies sum__allowances1;
+modifies Alloc;
+modifies sum__balances0;
+modifies M_Ref_int__balances0;
 procedure {:inline 1} send__success(from: Ref, to: Ref, amount: int) returns (success: bool);
 modifies __tmp__Balance;
 modifies __tmp__DType;
 modifies __tmp__Alloc;
 modifies __tmp__balance_ADDR;
-modifies __tmp__M_Ref_int;
-modifies __tmp__M_Ref_Ref;
+modifies __tmp__M_Ref_int__balances0;
+modifies __tmp__sum__balances0;
+modifies __tmp__M_Ref_int__allowances1;
+modifies __tmp__M_Ref_Ref__allowances1;
+modifies __tmp__sum__allowances1;
 modifies __tmp__Length;
+modifies __tmp__now;
 modifies __tmp___balances_ERC20;
 modifies __tmp___allowances_ERC20;
 modifies __tmp___totalSupply_ERC20;
 modifies revert;
 modifies gas;
 modifies Balance;
-modifies M_Ref_Ref;
-modifies M_Ref_int;
+modifies M_Ref_Ref__allowances1;
+modifies M_Ref_int__allowances1;
+modifies sum__allowances1;
 modifies Alloc;
-procedure BoogieEntry_Context();
-modifies gas;
-modifies revert;
-modifies __tmp__Balance;
-modifies __tmp__DType;
-modifies __tmp__Alloc;
-modifies __tmp__balance_ADDR;
-modifies __tmp__M_Ref_int;
-modifies __tmp__M_Ref_Ref;
-modifies __tmp__Length;
-modifies __tmp___balances_ERC20;
-modifies __tmp___allowances_ERC20;
-modifies __tmp___totalSupply_ERC20;
-procedure BoogieEntry_SafeMath();
-modifies gas;
-procedure BoogieEntry_IERC20();
-modifies gas;
-procedure BoogieEntry_ERC20();
-modifies gas;
-modifies _totalSupply_ERC20;
-modifies _balances_ERC20;
-modifies M_Ref_int;
-modifies _allowances_ERC20;
-modifies M_Ref_Ref;
-modifies Alloc;
-modifies revert;
-modifies __tmp__Balance;
-modifies __tmp__DType;
-modifies __tmp__Alloc;
-modifies __tmp__balance_ADDR;
-modifies __tmp__M_Ref_int;
-modifies __tmp__M_Ref_Ref;
-modifies __tmp__Length;
-modifies __tmp___balances_ERC20;
-modifies __tmp___allowances_ERC20;
-modifies __tmp___totalSupply_ERC20;
+modifies sum__balances0;
+modifies M_Ref_int__balances0;
 procedure CorralChoice_Context(this: Ref);
 modifies gas;
+modifies now;
+modifies Alloc;
 procedure CorralEntry_Context();
 modifies gas;
+modifies Alloc;
 modifies revert;
 modifies __tmp__Balance;
 modifies __tmp__DType;
 modifies __tmp__Alloc;
 modifies __tmp__balance_ADDR;
-modifies __tmp__M_Ref_int;
-modifies __tmp__M_Ref_Ref;
+modifies __tmp__M_Ref_int__balances0;
+modifies __tmp__sum__balances0;
+modifies __tmp__M_Ref_int__allowances1;
+modifies __tmp__M_Ref_Ref__allowances1;
+modifies __tmp__sum__allowances1;
 modifies __tmp__Length;
+modifies __tmp__now;
 modifies __tmp___balances_ERC20;
 modifies __tmp___allowances_ERC20;
 modifies __tmp___totalSupply_ERC20;
+modifies now;
+modifies Balance;
 procedure CorralChoice_SafeMath(this: Ref);
 modifies gas;
+modifies now;
+modifies Alloc;
 procedure CorralEntry_SafeMath();
 modifies gas;
+modifies Alloc;
+modifies Balance;
+modifies now;
 procedure CorralChoice_IERC20(this: Ref);
 modifies gas;
+modifies now;
+modifies Alloc;
 procedure CorralEntry_IERC20();
 modifies gas;
+modifies Alloc;
+modifies Balance;
+modifies now;
 procedure CorralChoice_ERC20(this: Ref);
 modifies gas;
+modifies now;
+modifies Alloc;
 modifies revert;
 modifies __tmp__Balance;
 modifies __tmp__DType;
 modifies __tmp__Alloc;
 modifies __tmp__balance_ADDR;
-modifies __tmp__M_Ref_int;
-modifies __tmp__M_Ref_Ref;
+modifies __tmp__M_Ref_int__balances0;
+modifies __tmp__sum__balances0;
+modifies __tmp__M_Ref_int__allowances1;
+modifies __tmp__M_Ref_Ref__allowances1;
+modifies __tmp__sum__allowances1;
 modifies __tmp__Length;
+modifies __tmp__now;
 modifies __tmp___balances_ERC20;
 modifies __tmp___allowances_ERC20;
 modifies __tmp___totalSupply_ERC20;
-modifies M_Ref_Ref;
-modifies M_Ref_int;
-modifies Alloc;
-procedure CorralEntry_ERC20();
+modifies M_Ref_Ref__allowances1;
+modifies M_Ref_int__allowances1;
+modifies sum__allowances1;
+modifies sum__balances0;
+modifies M_Ref_int__balances0;
+procedure main();
 modifies gas;
-modifies _totalSupply_ERC20;
-modifies _balances_ERC20;
-modifies M_Ref_int;
-modifies _allowances_ERC20;
-modifies M_Ref_Ref;
 modifies Alloc;
+modifies Balance;
+modifies _balances_ERC20;
+modifies M_Ref_int__balances0;
+modifies sum__balances0;
+modifies _allowances_ERC20;
+modifies M_Ref_Ref__allowances1;
+modifies M_Ref_int__allowances1;
+modifies _totalSupply_ERC20;
+modifies now;
 modifies revert;
 modifies __tmp__Balance;
 modifies __tmp__DType;
 modifies __tmp__Alloc;
 modifies __tmp__balance_ADDR;
-modifies __tmp__M_Ref_int;
-modifies __tmp__M_Ref_Ref;
+modifies __tmp__M_Ref_int__balances0;
+modifies __tmp__sum__balances0;
+modifies __tmp__M_Ref_int__allowances1;
+modifies __tmp__M_Ref_Ref__allowances1;
+modifies __tmp__sum__allowances1;
 modifies __tmp__Length;
+modifies __tmp__now;
 modifies __tmp___balances_ERC20;
 modifies __tmp___allowances_ERC20;
 modifies __tmp___totalSupply_ERC20;
+modifies sum__allowances1;
 var __tmp__Balance: [Ref]int;
 var __tmp__DType: [Ref]ContractName;
 var __tmp__Alloc: [Ref]bool;
 var __tmp__balance_ADDR: [Ref]int;
-var __tmp__M_Ref_int: [Ref][Ref]int;
-var __tmp__M_Ref_Ref: [Ref][Ref]Ref;
+var __tmp__M_Ref_int__balances0: [Ref][Ref]int;
+var __tmp__sum__balances0: [Ref]int;
+var __tmp__M_Ref_int__allowances1: [Ref][Ref]int;
+var __tmp__M_Ref_Ref__allowances1: [Ref][Ref]Ref;
+var __tmp__sum__allowances1: [Ref]int;
 var __tmp__Length: [Ref]int;
+var __tmp__now: int;
 var __tmp___balances_ERC20: [Ref]Ref;
 var __tmp___allowances_ERC20: [Ref]Ref;
 var __tmp___totalSupply_ERC20: [Ref]int;
 procedure {:inline 1} FreshRefGenerator__fail() returns (newRef: Ref);
 modifies __tmp__Alloc;
 procedure {:inline 1} Context_Context_NoBaseCtor__fail(this: Ref, msgsender_MSG: Ref, msgvalue_MSG: int);
+modifies __tmp__Balance;
 procedure {:constructor} {:inline 1} Context_Context__success(this: Ref, msgsender_MSG: Ref, msgvalue_MSG: int);
+modifies Balance;
 procedure {:constructor} {:inline 1} Context_Context__fail(this: Ref, msgsender_MSG: Ref, msgvalue_MSG: int);
+modifies __tmp__Balance;
 procedure {:inline 1} _msgSender_Context__fail(this: Ref, msgsender_MSG: Ref, msgvalue_MSG: int) returns (__ret_0_: Ref);
+modifies gas;
 procedure {:inline 1} SafeMath_SafeMath_NoBaseCtor__fail(this: Ref, msgsender_MSG: Ref, msgvalue_MSG: int);
+modifies __tmp__Balance;
 procedure {:inline 1} SafeMath_SafeMath__success(this: Ref, msgsender_MSG: Ref, msgvalue_MSG: int);
+modifies Balance;
 procedure {:inline 1} SafeMath_SafeMath__fail(this: Ref, msgsender_MSG: Ref, msgvalue_MSG: int);
+modifies __tmp__Balance;
 procedure {:inline 1} add_SafeMath__fail(this: Ref, msgsender_MSG: Ref, msgvalue_MSG: int, a_s40: int, b_s40: int) returns (__ret_0_: int);
+modifies gas;
 modifies revert;
 procedure {:inline 1} sub_SafeMath__fail(this: Ref, msgsender_MSG: Ref, msgvalue_MSG: int, a_s65: int, b_s65: int) returns (__ret_0_: int);
+modifies gas;
 modifies revert;
 procedure {:inline 1} mul_SafeMath__fail(this: Ref, msgsender_MSG: Ref, msgvalue_MSG: int, a_s99: int, b_s99: int) returns (__ret_0_: int);
 modifies revert;
@@ -721,158 +916,238 @@ modifies revert;
 procedure {:inline 1} mod_SafeMath__fail(this: Ref, msgsender_MSG: Ref, msgvalue_MSG: int, a_s145: int, b_s145: int) returns (__ret_0_: int);
 modifies revert;
 procedure {:inline 1} IERC20_IERC20_NoBaseCtor__fail(this: Ref, msgsender_MSG: Ref, msgvalue_MSG: int);
+modifies __tmp__Balance;
 procedure {:inline 1} IERC20_IERC20__success(this: Ref, msgsender_MSG: Ref, msgvalue_MSG: int);
+modifies Balance;
 procedure {:inline 1} IERC20_IERC20__fail(this: Ref, msgsender_MSG: Ref, msgvalue_MSG: int);
+modifies __tmp__Balance;
 procedure {:inline 1} ERC20_ERC20_NoBaseCtor__fail(this: Ref, msgsender_MSG: Ref, msgvalue_MSG: int);
-modifies __tmp___totalSupply_ERC20;
+modifies __tmp__Balance;
 modifies __tmp___balances_ERC20;
-modifies __tmp__M_Ref_int;
+modifies __tmp__M_Ref_int__balances0;
+modifies __tmp__sum__balances0;
 modifies __tmp___allowances_ERC20;
-modifies __tmp__M_Ref_Ref;
+modifies __tmp__M_Ref_Ref__allowances1;
+modifies __tmp__M_Ref_int__allowances1;
+modifies __tmp___totalSupply_ERC20;
 modifies __tmp__Alloc;
 procedure {:inline 1} ERC20_ERC20__success(this: Ref, msgsender_MSG: Ref, msgvalue_MSG: int);
-modifies _totalSupply_ERC20;
+modifies Balance;
 modifies _balances_ERC20;
-modifies M_Ref_int;
+modifies M_Ref_int__balances0;
+modifies sum__balances0;
 modifies _allowances_ERC20;
-modifies M_Ref_Ref;
+modifies M_Ref_Ref__allowances1;
+modifies M_Ref_int__allowances1;
+modifies _totalSupply_ERC20;
 modifies Alloc;
 procedure {:inline 1} ERC20_ERC20__fail(this: Ref, msgsender_MSG: Ref, msgvalue_MSG: int);
-modifies __tmp___totalSupply_ERC20;
+modifies __tmp__Balance;
 modifies __tmp___balances_ERC20;
-modifies __tmp__M_Ref_int;
+modifies __tmp__M_Ref_int__balances0;
+modifies __tmp__sum__balances0;
 modifies __tmp___allowances_ERC20;
-modifies __tmp__M_Ref_Ref;
+modifies __tmp__M_Ref_Ref__allowances1;
+modifies __tmp__M_Ref_int__allowances1;
+modifies __tmp___totalSupply_ERC20;
 modifies __tmp__Alloc;
 procedure {:inline 1} totalSupply_ERC20__success(this: Ref, msgsender_MSG: Ref, msgvalue_MSG: int) returns (__ret_0_: int);
+modifies gas;
 procedure {:inline 1} totalSupply_ERC20__fail(this: Ref, msgsender_MSG: Ref, msgvalue_MSG: int) returns (__ret_0_: int);
+modifies gas;
 procedure {:inline 1} balanceOf_ERC20__success(this: Ref, msgsender_MSG: Ref, msgvalue_MSG: int, account_s252: Ref) returns (__ret_0_: int);
+modifies gas;
 procedure {:inline 1} balanceOf_ERC20__fail(this: Ref, msgsender_MSG: Ref, msgvalue_MSG: int, account_s252: Ref) returns (__ret_0_: int);
+modifies gas;
 procedure {:inline 1} transfer_ERC20__success(this: Ref, msgsender_MSG: Ref, msgvalue_MSG: int, recipient_s267: Ref, amount_s267: int) returns (__ret_0_: bool);
+modifies gas;
 modifies revert;
-modifies M_Ref_int;
+modifies sum__balances0;
+modifies M_Ref_int__balances0;
 procedure {:inline 1} transfer_ERC20__fail(this: Ref, msgsender_MSG: Ref, msgvalue_MSG: int, recipient_s267: Ref, amount_s267: int) returns (__ret_0_: bool);
+modifies gas;
 modifies revert;
-modifies __tmp__M_Ref_int;
+modifies __tmp__sum__balances0;
+modifies __tmp__M_Ref_int__balances0;
 procedure {:inline 1} transfer_ERC20_ERC20__fail(this: Ref, msgsender_MSG: Ref, msgvalue_MSG: int, recipient_s286: Ref, amount_s286: int) returns (__ret_0_: bool);
+modifies gas;
 modifies revert;
-modifies __tmp__M_Ref_int;
+modifies __tmp__sum__balances0;
+modifies __tmp__M_Ref_int__balances0;
 procedure {:inline 1} allowance_ERC20__success(this: Ref, msgsender_MSG: Ref, msgvalue_MSG: int, owner_s302: Ref, spender_s302: Ref) returns (__ret_0_: int);
-modifies M_Ref_Ref;
-modifies M_Ref_int;
+modifies gas;
+modifies M_Ref_Ref__allowances1;
+modifies M_Ref_int__allowances1;
+modifies sum__allowances1;
 modifies Alloc;
 procedure {:inline 1} allowance_ERC20__fail(this: Ref, msgsender_MSG: Ref, msgvalue_MSG: int, owner_s302: Ref, spender_s302: Ref) returns (__ret_0_: int);
-modifies __tmp__M_Ref_Ref;
-modifies __tmp__M_Ref_int;
+modifies gas;
+modifies __tmp__M_Ref_Ref__allowances1;
+modifies __tmp__M_Ref_int__allowances1;
+modifies __tmp__sum__allowances1;
 modifies __tmp__Alloc;
 procedure {:inline 1} approve_ERC20__success(this: Ref, msgsender_MSG: Ref, msgvalue_MSG: int, spender_s317: Ref, amount_s317: int) returns (__ret_0_: bool);
+modifies gas;
 modifies revert;
-modifies M_Ref_Ref;
-modifies M_Ref_int;
+modifies M_Ref_Ref__allowances1;
+modifies M_Ref_int__allowances1;
+modifies sum__allowances1;
 modifies Alloc;
 procedure {:inline 1} approve_ERC20__fail(this: Ref, msgsender_MSG: Ref, msgvalue_MSG: int, spender_s317: Ref, amount_s317: int) returns (__ret_0_: bool);
+modifies gas;
 modifies revert;
-modifies __tmp__M_Ref_Ref;
-modifies __tmp__M_Ref_int;
+modifies __tmp__M_Ref_Ref__allowances1;
+modifies __tmp__M_Ref_int__allowances1;
+modifies __tmp__sum__allowances1;
 modifies __tmp__Alloc;
 procedure {:inline 1} approve_ERC20_ERC20__fail(this: Ref, msgsender_MSG: Ref, msgvalue_MSG: int, spender_s336: Ref, amount_s336: int) returns (__ret_0_: bool);
+modifies gas;
 modifies revert;
-modifies __tmp__M_Ref_Ref;
-modifies __tmp__M_Ref_int;
+modifies __tmp__M_Ref_Ref__allowances1;
+modifies __tmp__M_Ref_int__allowances1;
+modifies __tmp__sum__allowances1;
 modifies __tmp__Alloc;
 procedure {:inline 1} transferFrom_ERC20__success(this: Ref, msgsender_MSG: Ref, msgvalue_MSG: int, sender_s354: Ref, recipient_s354: Ref, amount_s354: int) returns (__ret_0_: bool);
-modifies M_Ref_Ref;
-modifies M_Ref_int;
+modifies gas;
+modifies M_Ref_Ref__allowances1;
+modifies M_Ref_int__allowances1;
+modifies sum__allowances1;
 modifies revert;
+modifies sum__balances0;
+modifies M_Ref_int__balances0;
 modifies Alloc;
 procedure {:inline 1} transferFrom_ERC20__fail(this: Ref, msgsender_MSG: Ref, msgvalue_MSG: int, sender_s354: Ref, recipient_s354: Ref, amount_s354: int) returns (__ret_0_: bool);
-modifies __tmp__M_Ref_Ref;
-modifies __tmp__M_Ref_int;
+modifies gas;
+modifies __tmp__M_Ref_Ref__allowances1;
+modifies __tmp__M_Ref_int__allowances1;
+modifies __tmp__sum__allowances1;
 modifies revert;
+modifies __tmp__sum__balances0;
+modifies __tmp__M_Ref_int__balances0;
 modifies __tmp__Alloc;
 procedure {:inline 1} transferFrom_ERC20_ERC20__fail(this: Ref, msgsender_MSG: Ref, msgvalue_MSG: int, sender_s389: Ref, recipient_s389: Ref, amount_s389: int) returns (__ret_0_: bool);
-modifies __tmp__M_Ref_Ref;
-modifies __tmp__M_Ref_int;
+modifies gas;
+modifies __tmp__M_Ref_Ref__allowances1;
+modifies __tmp__M_Ref_int__allowances1;
+modifies __tmp__sum__allowances1;
 modifies revert;
+modifies __tmp__sum__balances0;
+modifies __tmp__M_Ref_int__balances0;
 modifies __tmp__Alloc;
 procedure {:inline 1} increaseAllowance_ERC20__success(this: Ref, msgsender_MSG: Ref, msgvalue_MSG: int, spender_s404: Ref, addedValue_s404: int) returns (__ret_0_: bool);
-modifies M_Ref_Ref;
-modifies M_Ref_int;
+modifies gas;
+modifies M_Ref_Ref__allowances1;
+modifies M_Ref_int__allowances1;
+modifies sum__allowances1;
 modifies Alloc;
 modifies revert;
 procedure {:inline 1} increaseAllowance_ERC20__fail(this: Ref, msgsender_MSG: Ref, msgvalue_MSG: int, spender_s404: Ref, addedValue_s404: int) returns (__ret_0_: bool);
-modifies __tmp__M_Ref_Ref;
-modifies __tmp__M_Ref_int;
+modifies gas;
+modifies __tmp__M_Ref_Ref__allowances1;
+modifies __tmp__M_Ref_int__allowances1;
+modifies __tmp__sum__allowances1;
 modifies __tmp__Alloc;
 modifies revert;
 procedure {:inline 1} increaseAllowance_ERC20_ERC20__fail(this: Ref, msgsender_MSG: Ref, msgvalue_MSG: int, spender_s431: Ref, addedValue_s431: int) returns (__ret_0_: bool);
-modifies __tmp__M_Ref_Ref;
-modifies __tmp__M_Ref_int;
+modifies gas;
+modifies __tmp__M_Ref_Ref__allowances1;
+modifies __tmp__M_Ref_int__allowances1;
+modifies __tmp__sum__allowances1;
 modifies __tmp__Alloc;
 modifies revert;
 procedure {:inline 1} decreaseAllowance_ERC20__success(this: Ref, msgsender_MSG: Ref, msgvalue_MSG: int, spender_s446: Ref, subtractedValue_s446: int) returns (__ret_0_: bool);
-modifies M_Ref_Ref;
-modifies M_Ref_int;
+modifies gas;
+modifies M_Ref_Ref__allowances1;
+modifies M_Ref_int__allowances1;
+modifies sum__allowances1;
 modifies Alloc;
 modifies revert;
 procedure {:inline 1} decreaseAllowance_ERC20__fail(this: Ref, msgsender_MSG: Ref, msgvalue_MSG: int, spender_s446: Ref, subtractedValue_s446: int) returns (__ret_0_: bool);
-modifies __tmp__M_Ref_Ref;
-modifies __tmp__M_Ref_int;
+modifies gas;
+modifies __tmp__M_Ref_Ref__allowances1;
+modifies __tmp__M_Ref_int__allowances1;
+modifies __tmp__sum__allowances1;
 modifies __tmp__Alloc;
 modifies revert;
 procedure {:inline 1} decreaseAllowance_ERC20_ERC20__fail(this: Ref, msgsender_MSG: Ref, msgvalue_MSG: int, spender_s473: Ref, subtractedValue_s473: int) returns (__ret_0_: bool);
-modifies __tmp__M_Ref_Ref;
-modifies __tmp__M_Ref_int;
+modifies gas;
+modifies __tmp__M_Ref_Ref__allowances1;
+modifies __tmp__M_Ref_int__allowances1;
+modifies __tmp__sum__allowances1;
 modifies __tmp__Alloc;
 modifies revert;
 procedure {:inline 1} _transfer_ERC20__fail(this: Ref, msgsender_MSG: Ref, msgvalue_MSG: int, sender_s529: Ref, recipient_s529: Ref, amount_s529: int);
+modifies gas;
 modifies revert;
-modifies __tmp__M_Ref_int;
+modifies __tmp__sum__balances0;
+modifies __tmp__M_Ref_int__balances0;
 procedure {:inline 1} _mint_ERC20__fail(this: Ref, msgsender_MSG: Ref, msgvalue_MSG: int, account_s542: Ref, amount_s542: int);
 modifies revert;
 modifies __tmp___totalSupply_ERC20;
-modifies __tmp__M_Ref_int;
+modifies __tmp__sum__balances0;
+modifies __tmp__M_Ref_int__balances0;
+modifies gas;
 procedure {:inline 1} _mint_ERC20_ERC20__fail(this: Ref, msgsender_MSG: Ref, msgvalue_MSG: int, account_s585: Ref, amount_s585: int);
 modifies revert;
 modifies __tmp___totalSupply_ERC20;
-modifies __tmp__M_Ref_int;
+modifies __tmp__sum__balances0;
+modifies __tmp__M_Ref_int__balances0;
+modifies gas;
 procedure {:inline 1} _burn_ERC20__fail(this: Ref, msgsender_MSG: Ref, msgvalue_MSG: int, account_s628: Ref, amount_s628: int);
 modifies revert;
-modifies __tmp__M_Ref_int;
+modifies __tmp__sum__balances0;
+modifies __tmp__M_Ref_int__balances0;
 modifies __tmp___totalSupply_ERC20;
+modifies gas;
 procedure {:inline 1} _approve_ERC20__fail(this: Ref, msgsender_MSG: Ref, msgvalue_MSG: int, owner_s670: Ref, spender_s670: Ref, amount_s670: int);
+modifies gas;
 modifies revert;
-modifies __tmp__M_Ref_Ref;
-modifies __tmp__M_Ref_int;
+modifies __tmp__M_Ref_Ref__allowances1;
+modifies __tmp__M_Ref_int__allowances1;
+modifies __tmp__sum__allowances1;
 modifies __tmp__Alloc;
 procedure {:inline 1} _burnFrom_ERC20__fail(this: Ref, msgsender_MSG: Ref, msgvalue_MSG: int, account_s698: Ref, amount_s698: int);
-modifies __tmp__M_Ref_Ref;
-modifies __tmp__M_Ref_int;
+modifies __tmp__M_Ref_Ref__allowances1;
+modifies __tmp__M_Ref_int__allowances1;
+modifies __tmp__sum__allowances1;
 modifies revert;
+modifies __tmp__sum__balances0;
+modifies __tmp__M_Ref_int__balances0;
 modifies __tmp___totalSupply_ERC20;
+modifies gas;
 modifies __tmp__Alloc;
 procedure {:inline 1} FallbackDispatch__fail(from: Ref, to: Ref, amount: int);
 modifies __tmp__Balance;
-modifies gas;
-modifies __tmp__M_Ref_Ref;
-modifies __tmp__M_Ref_int;
-modifies __tmp__Alloc;
 modifies revert;
+modifies gas;
+modifies __tmp__M_Ref_Ref__allowances1;
+modifies __tmp__M_Ref_int__allowances1;
+modifies __tmp__sum__allowances1;
+modifies __tmp__Alloc;
+modifies __tmp__sum__balances0;
+modifies __tmp__M_Ref_int__balances0;
 procedure {:inline 1} Fallback_UnknownType__fail(from: Ref, to: Ref, amount: int);
 modifies __tmp__Balance;
-modifies gas;
-modifies __tmp__M_Ref_Ref;
-modifies __tmp__M_Ref_int;
-modifies __tmp__Alloc;
 modifies revert;
+modifies gas;
+modifies __tmp__M_Ref_Ref__allowances1;
+modifies __tmp__M_Ref_int__allowances1;
+modifies __tmp__sum__allowances1;
+modifies __tmp__Alloc;
+modifies __tmp__sum__balances0;
+modifies __tmp__M_Ref_int__balances0;
 procedure {:inline 1} send__fail(from: Ref, to: Ref, amount: int) returns (success: bool);
 modifies __tmp__Balance;
 modifies __tmp__DType;
 modifies __tmp__Alloc;
 modifies __tmp__balance_ADDR;
-modifies __tmp__M_Ref_int;
-modifies __tmp__M_Ref_Ref;
+modifies __tmp__M_Ref_int__balances0;
+modifies __tmp__sum__balances0;
+modifies __tmp__M_Ref_int__allowances1;
+modifies __tmp__M_Ref_Ref__allowances1;
+modifies __tmp__sum__allowances1;
 modifies __tmp__Length;
+modifies __tmp__now;
 modifies __tmp___balances_ERC20;
 modifies __tmp___allowances_ERC20;
 modifies __tmp___totalSupply_ERC20;
@@ -898,6 +1173,7 @@ implementation Context_Context_NoBaseCtor__fail(this: Ref, msgsender_MSG: Ref, m
 {
 // start of initialization
 assume ((msgsender_MSG) != (null));
+__tmp__Balance[this] := 0;
 // end of initialization
 }
 
@@ -905,6 +1181,7 @@ implementation Context_Context_NoBaseCtor__success(this: Ref, msgsender_MSG: Ref
 {
 // start of initialization
 assume ((msgsender_MSG) != (null));
+Balance[this] := 0;
 // end of initialization
 }
 
@@ -926,12 +1203,16 @@ return;
 
 implementation _msgSender_Context__fail(this: Ref, msgsender_MSG: Ref, msgvalue_MSG: int) returns (__ret_0_: Ref)
 {
+gas := (gas) - (3);
+gas := (gas) - (7);
 __ret_0_ := msgsender_MSG;
 return;
 }
 
 implementation _msgSender_Context__success(this: Ref, msgsender_MSG: Ref, msgvalue_MSG: int) returns (__ret_0_: Ref)
 {
+gas := (gas) - (3);
+gas := (gas) - (7);
 __ret_0_ := msgsender_MSG;
 return;
 }
@@ -940,6 +1221,7 @@ implementation SafeMath_SafeMath_NoBaseCtor__fail(this: Ref, msgsender_MSG: Ref,
 {
 // start of initialization
 assume ((msgsender_MSG) != (null));
+__tmp__Balance[this] := 0;
 // end of initialization
 }
 
@@ -947,6 +1229,7 @@ implementation SafeMath_SafeMath_NoBaseCtor__success(this: Ref, msgsender_MSG: R
 {
 // start of initialization
 assume ((msgsender_MSG) != (null));
+Balance[this] := 0;
 // end of initialization
 }
 
@@ -969,17 +1252,21 @@ return;
 implementation add_SafeMath__fail(this: Ref, msgsender_MSG: Ref, msgvalue_MSG: int, a_s40: int, b_s40: int) returns (__ret_0_: int)
 {
 var c_s39: int;
+gas := (gas) - (3);
+gas := (gas) - (17);
 assume ((c_s39) >= (0));
 assume ((a_s40) >= (0));
 assume ((b_s40) >= (0));
 assume (((a_s40) + (b_s40)) >= (0));
 c_s39 := (a_s40) + (b_s40);
+gas := (gas) - (664);
 assume ((c_s39) >= (0));
 assume ((a_s40) >= (0));
 if (!((c_s39) >= (a_s40))) {
 revert := true;
 return;
 }
+gas := (gas) - (10);
 assume ((c_s39) >= (0));
 __ret_0_ := c_s39;
 return;
@@ -988,17 +1275,21 @@ return;
 implementation add_SafeMath__success(this: Ref, msgsender_MSG: Ref, msgvalue_MSG: int, a_s40: int, b_s40: int) returns (__ret_0_: int)
 {
 var c_s39: int;
+gas := (gas) - (3);
+gas := (gas) - (17);
 assume ((c_s39) >= (0));
 assume ((a_s40) >= (0));
 assume ((b_s40) >= (0));
 assume (((a_s40) + (b_s40)) >= (0));
 c_s39 := (a_s40) + (b_s40);
+gas := (gas) - (664);
 assume ((c_s39) >= (0));
 assume ((a_s40) >= (0));
 if (!((c_s39) >= (a_s40))) {
 revert := true;
 return;
 }
+gas := (gas) - (10);
 assume ((c_s39) >= (0));
 __ret_0_ := c_s39;
 return;
@@ -1007,17 +1298,21 @@ return;
 implementation sub_SafeMath__fail(this: Ref, msgsender_MSG: Ref, msgvalue_MSG: int, a_s65: int, b_s65: int) returns (__ret_0_: int)
 {
 var c_s64: int;
+gas := (gas) - (3);
+gas := (gas) - (664);
 assume ((b_s65) >= (0));
 assume ((a_s65) >= (0));
 if (!((b_s65) <= (a_s65))) {
 revert := true;
 return;
 }
+gas := (gas) - (17);
 assume ((c_s64) >= (0));
 assume ((a_s65) >= (0));
 assume ((b_s65) >= (0));
 assume (((a_s65) - (b_s65)) >= (0));
 c_s64 := (a_s65) - (b_s65);
+gas := (gas) - (10);
 assume ((c_s64) >= (0));
 __ret_0_ := c_s64;
 return;
@@ -1026,17 +1321,21 @@ return;
 implementation sub_SafeMath__success(this: Ref, msgsender_MSG: Ref, msgvalue_MSG: int, a_s65: int, b_s65: int) returns (__ret_0_: int)
 {
 var c_s64: int;
+gas := (gas) - (3);
+gas := (gas) - (664);
 assume ((b_s65) >= (0));
 assume ((a_s65) >= (0));
 if (!((b_s65) <= (a_s65))) {
 revert := true;
 return;
 }
+gas := (gas) - (17);
 assume ((c_s64) >= (0));
 assume ((a_s65) >= (0));
 assume ((b_s65) >= (0));
 assume (((a_s65) - (b_s65)) >= (0));
 c_s64 := (a_s65) - (b_s65);
+gas := (gas) - (10);
 assume ((c_s64) >= (0));
 __ret_0_ := c_s64;
 return;
@@ -1053,13 +1352,13 @@ return;
 assume ((c_s98) >= (0));
 assume ((a_s99) >= (0));
 assume ((b_s99) >= (0));
-assume (((a_s99) * (b_s99)) >= (0));
-c_s98 := (a_s99) * (b_s99);
+assume ((nonlinearMul(a_s99, b_s99)) >= (0));
+c_s98 := nonlinearMul(a_s99, b_s99);
 assume ((c_s98) >= (0));
 assume ((a_s99) >= (0));
-assume (((c_s98) / (a_s99)) >= (0));
+assume ((nonlinearDiv(c_s98, a_s99)) >= (0));
 assume ((b_s99) >= (0));
-if (!(((c_s98) / (a_s99)) == (b_s99))) {
+if (!((nonlinearDiv(c_s98, a_s99)) == (b_s99))) {
 revert := true;
 return;
 }
@@ -1079,13 +1378,13 @@ return;
 assume ((c_s98) >= (0));
 assume ((a_s99) >= (0));
 assume ((b_s99) >= (0));
-assume (((a_s99) * (b_s99)) >= (0));
-c_s98 := (a_s99) * (b_s99);
+assume ((nonlinearMul(a_s99, b_s99)) >= (0));
+c_s98 := nonlinearMul(a_s99, b_s99);
 assume ((c_s98) >= (0));
 assume ((a_s99) >= (0));
-assume (((c_s98) / (a_s99)) >= (0));
+assume ((nonlinearDiv(c_s98, a_s99)) >= (0));
 assume ((b_s99) >= (0));
-if (!(((c_s98) / (a_s99)) == (b_s99))) {
+if (!((nonlinearDiv(c_s98, a_s99)) == (b_s99))) {
 revert := true;
 return;
 }
@@ -1094,11 +1393,75 @@ __ret_0_ := c_s98;
 return;
 }
 
+implementation div_SafeMath__fail(this: Ref, msgsender_MSG: Ref, msgvalue_MSG: int, a_s124: int, b_s124: int) returns (__ret_0_: int)
+{
+var c_s123: int;
+assume ((b_s124) >= (0));
+if (!((b_s124) > (0))) {
+revert := true;
+return;
+}
+assume ((c_s123) >= (0));
+assume ((a_s124) >= (0));
+assume ((b_s124) >= (0));
+assume ((nonlinearDiv(a_s124, b_s124)) >= (0));
+c_s123 := nonlinearDiv(a_s124, b_s124);
+assume ((c_s123) >= (0));
+__ret_0_ := c_s123;
+return;
+}
+
+implementation div_SafeMath__success(this: Ref, msgsender_MSG: Ref, msgvalue_MSG: int, a_s124: int, b_s124: int) returns (__ret_0_: int)
+{
+var c_s123: int;
+assume ((b_s124) >= (0));
+if (!((b_s124) > (0))) {
+revert := true;
+return;
+}
+assume ((c_s123) >= (0));
+assume ((a_s124) >= (0));
+assume ((b_s124) >= (0));
+assume ((nonlinearDiv(a_s124, b_s124)) >= (0));
+c_s123 := nonlinearDiv(a_s124, b_s124);
+assume ((c_s123) >= (0));
+__ret_0_ := c_s123;
+return;
+}
+
+implementation mod_SafeMath__fail(this: Ref, msgsender_MSG: Ref, msgvalue_MSG: int, a_s145: int, b_s145: int) returns (__ret_0_: int)
+{
+assume ((b_s145) >= (0));
+if (!((b_s145) != (0))) {
+revert := true;
+return;
+}
+assume ((a_s145) >= (0));
+assume ((b_s145) >= (0));
+assume ((nonlinearMod(a_s145, b_s145)) >= (0));
+__ret_0_ := nonlinearMod(a_s145, b_s145);
+return;
+}
+
+implementation mod_SafeMath__success(this: Ref, msgsender_MSG: Ref, msgvalue_MSG: int, a_s145: int, b_s145: int) returns (__ret_0_: int)
+{
+assume ((b_s145) >= (0));
+if (!((b_s145) != (0))) {
+revert := true;
+return;
+}
+assume ((a_s145) >= (0));
+assume ((b_s145) >= (0));
+assume ((nonlinearMod(a_s145, b_s145)) >= (0));
+__ret_0_ := nonlinearMod(a_s145, b_s145);
+return;
+}
 
 implementation IERC20_IERC20_NoBaseCtor__fail(this: Ref, msgsender_MSG: Ref, msgvalue_MSG: int)
 {
 // start of initialization
 assume ((msgsender_MSG) != (null));
+__tmp__Balance[this] := 0;
 // end of initialization
 }
 
@@ -1106,6 +1469,7 @@ implementation IERC20_IERC20_NoBaseCtor__success(this: Ref, msgsender_MSG: Ref, 
 {
 // start of initialization
 assume ((msgsender_MSG) != (null));
+Balance[this] := 0;
 // end of initialization
 }
 
@@ -1131,7 +1495,7 @@ var __var_1: Ref;
 var __var_2: Ref;
 // start of initialization
 assume ((msgsender_MSG) != (null));
-__tmp___totalSupply_ERC20[this] := 0;
+__tmp__Balance[this] := 0;
 // Make array/mapping vars distinct for _balances
 call __var_1 := FreshRefGenerator__fail();
 if (revert) {
@@ -1139,7 +1503,8 @@ return;
 }
 __tmp___balances_ERC20[this] := __var_1;
 // Initialize Integer mapping _balances
-__tmp__M_Ref_int[__tmp___balances_ERC20[this]] := zeroRefIntArr();
+__tmp__M_Ref_int__balances0[__tmp___balances_ERC20[this]] := zeroRefIntArr();
+__tmp__sum__balances0[__tmp___balances_ERC20[this]] := 0;
 // Make array/mapping vars distinct for _allowances
 call __var_2 := FreshRefGenerator__fail();
 if (revert) {
@@ -1147,7 +1512,9 @@ return;
 }
 __tmp___allowances_ERC20[this] := __var_2;
 // Initialize length of 1-level nested array in _allowances
-__tmp__M_Ref_Ref[__tmp___allowances_ERC20[this]] := zeroRefRefArr();
+__tmp__M_Ref_Ref__allowances1[__tmp___allowances_ERC20[this]] := zeroRefRefArr();
+__tmp__M_Ref_int__allowances1[null] := zeroRefIntArr();
+__tmp___totalSupply_ERC20[this] := 0;
 // end of initialization
 }
 
@@ -1157,7 +1524,7 @@ var __var_1: Ref;
 var __var_2: Ref;
 // start of initialization
 assume ((msgsender_MSG) != (null));
-_totalSupply_ERC20[this] := 0;
+Balance[this] := 0;
 // Make array/mapping vars distinct for _balances
 call __var_1 := FreshRefGenerator__success();
 if (revert) {
@@ -1165,7 +1532,8 @@ return;
 }
 _balances_ERC20[this] := __var_1;
 // Initialize Integer mapping _balances
-M_Ref_int[_balances_ERC20[this]] := zeroRefIntArr();
+M_Ref_int__balances0[_balances_ERC20[this]] := zeroRefIntArr();
+sum__balances0[_balances_ERC20[this]] := 0;
 // Make array/mapping vars distinct for _allowances
 call __var_2 := FreshRefGenerator__success();
 if (revert) {
@@ -1173,7 +1541,9 @@ return;
 }
 _allowances_ERC20[this] := __var_2;
 // Initialize length of 1-level nested array in _allowances
-M_Ref_Ref[_allowances_ERC20[this]] := zeroRefRefArr();
+M_Ref_Ref__allowances1[_allowances_ERC20[this]] := zeroRefRefArr();
+M_Ref_int__allowances1[null] := zeroRefIntArr();
+_totalSupply_ERC20[this] := 0;
 // end of initialization
 }
 
@@ -1211,6 +1581,8 @@ return;
 
 implementation totalSupply_ERC20__fail(this: Ref, msgsender_MSG: Ref, msgvalue_MSG: int) returns (__ret_0_: int)
 {
+gas := (gas) - (3);
+gas := (gas) - (208);
 assume ((__tmp___totalSupply_ERC20[this]) >= (0));
 __ret_0_ := __tmp___totalSupply_ERC20[this];
 return;
@@ -1218,6 +1590,8 @@ return;
 
 implementation totalSupply_ERC20__success(this: Ref, msgsender_MSG: Ref, msgvalue_MSG: int) returns (__ret_0_: int)
 {
+gas := (gas) - (3);
+gas := (gas) - (208);
 assume ((_totalSupply_ERC20[this]) >= (0));
 __ret_0_ := _totalSupply_ERC20[this];
 return;
@@ -1225,21 +1599,27 @@ return;
 
 implementation balanceOf_ERC20__fail(this: Ref, msgsender_MSG: Ref, msgvalue_MSG: int, account_s252: Ref) returns (__ret_0_: int)
 {
-assume ((__tmp__M_Ref_int[__tmp___balances_ERC20[this]][account_s252]) >= (0));
-__ret_0_ := __tmp__M_Ref_int[__tmp___balances_ERC20[this]][account_s252];
+gas := (gas) - (3);
+gas := (gas) - (304);
+assume ((__tmp__M_Ref_int__balances0[__tmp___balances_ERC20[this]][account_s252]) >= (0));
+__ret_0_ := __tmp__M_Ref_int__balances0[__tmp___balances_ERC20[this]][account_s252];
 return;
 }
 
 implementation balanceOf_ERC20__success(this: Ref, msgsender_MSG: Ref, msgvalue_MSG: int, account_s252: Ref) returns (__ret_0_: int)
 {
-assume ((M_Ref_int[_balances_ERC20[this]][account_s252]) >= (0));
-__ret_0_ := M_Ref_int[_balances_ERC20[this]][account_s252];
+gas := (gas) - (3);
+gas := (gas) - (304);
+assume ((M_Ref_int__balances0[_balances_ERC20[this]][account_s252]) >= (0));
+__ret_0_ := M_Ref_int__balances0[_balances_ERC20[this]][account_s252];
 return;
 }
 
 implementation transfer_ERC20__fail(this: Ref, msgsender_MSG: Ref, msgvalue_MSG: int, recipient_s267: Ref, amount_s267: int) returns (__ret_0_: bool)
 {
 var __var_3: bool;
+gas := (gas) - (3);
+gas := (gas) - (15);
 assume ((amount_s267) >= (0));
 call __var_3 := transfer_ERC20_ERC20__fail(this, msgsender_MSG, msgvalue_MSG, recipient_s267, amount_s267);
 if (revert) {
@@ -1252,6 +1632,8 @@ return;
 implementation transfer_ERC20__success(this: Ref, msgsender_MSG: Ref, msgvalue_MSG: int, recipient_s267: Ref, amount_s267: int) returns (__ret_0_: bool)
 {
 var __var_3: bool;
+gas := (gas) - (3);
+gas := (gas) - (15);
 assume ((amount_s267) >= (0));
 call __var_3 := transfer_ERC20_ERC20__success(this, msgsender_MSG, msgvalue_MSG, recipient_s267, amount_s267);
 if (revert) {
@@ -1264,6 +1646,8 @@ return;
 implementation transfer_ERC20_ERC20__fail(this: Ref, msgsender_MSG: Ref, msgvalue_MSG: int, recipient_s286: Ref, amount_s286: int) returns (__ret_0_: bool)
 {
 var __var_4: Ref;
+gas := (gas) - (3);
+gas := (gas) - (36);
 if ((__tmp__DType[this]) == (ERC20)) {
 call __var_4 := _msgSender_Context__fail(this, msgsender_MSG, msgvalue_MSG);
 if (revert) {
@@ -1277,6 +1661,7 @@ call _transfer_ERC20__fail(this, msgsender_MSG, msgvalue_MSG, __var_4, recipient
 if (revert) {
 return;
 }
+gas := (gas) - (8);
 __ret_0_ := true;
 return;
 }
@@ -1284,6 +1669,8 @@ return;
 implementation transfer_ERC20_ERC20__success(this: Ref, msgsender_MSG: Ref, msgvalue_MSG: int, recipient_s286: Ref, amount_s286: int) returns (__ret_0_: bool)
 {
 var __var_4: Ref;
+gas := (gas) - (3);
+gas := (gas) - (36);
 if ((DType[this]) == (ERC20)) {
 call __var_4 := _msgSender_Context__success(this, msgsender_MSG, msgvalue_MSG);
 if (revert) {
@@ -1297,6 +1684,7 @@ call _transfer_ERC20__success(this, msgsender_MSG, msgvalue_MSG, __var_4, recipi
 if (revert) {
 return;
 }
+gas := (gas) - (8);
 __ret_0_ := true;
 return;
 }
@@ -1304,38 +1692,46 @@ return;
 implementation allowance_ERC20__fail(this: Ref, msgsender_MSG: Ref, msgvalue_MSG: int, owner_s302: Ref, spender_s302: Ref) returns (__ret_0_: int)
 {
 var __var_5: Ref;
-if ((__tmp__M_Ref_Ref[__tmp___allowances_ERC20[this]][owner_s302]) == (null)) {
+gas := (gas) - (3);
+gas := (gas) - (394);
+if ((__tmp__M_Ref_Ref__allowances1[__tmp___allowances_ERC20[this]][owner_s302]) == (null)) {
 call __var_5 := FreshRefGenerator__fail();
 if (revert) {
 return;
 }
-__tmp__M_Ref_Ref[__tmp___allowances_ERC20[this]][owner_s302] := __var_5;
-__tmp__M_Ref_int[__tmp__M_Ref_Ref[__tmp___allowances_ERC20[this]][owner_s302]] := zeroRefIntArr();
+__tmp__M_Ref_Ref__allowances1[__tmp___allowances_ERC20[this]][owner_s302] := __var_5;
+__tmp__M_Ref_int__allowances1[__tmp__M_Ref_Ref__allowances1[__tmp___allowances_ERC20[this]][owner_s302]] := zeroRefIntArr();
+__tmp__sum__allowances1[__tmp__M_Ref_Ref__allowances1[__tmp___allowances_ERC20[this]][owner_s302]] := 0;
 }
-assume ((__tmp__M_Ref_int[__tmp__M_Ref_Ref[__tmp___allowances_ERC20[this]][owner_s302]][spender_s302]) >= (0));
-__ret_0_ := __tmp__M_Ref_int[__tmp__M_Ref_Ref[__tmp___allowances_ERC20[this]][owner_s302]][spender_s302];
+assume ((__tmp__M_Ref_int__allowances1[__tmp__M_Ref_Ref__allowances1[__tmp___allowances_ERC20[this]][owner_s302]][spender_s302]) >= (0));
+__ret_0_ := __tmp__M_Ref_int__allowances1[__tmp__M_Ref_Ref__allowances1[__tmp___allowances_ERC20[this]][owner_s302]][spender_s302];
 return;
 }
 
 implementation allowance_ERC20__success(this: Ref, msgsender_MSG: Ref, msgvalue_MSG: int, owner_s302: Ref, spender_s302: Ref) returns (__ret_0_: int)
 {
 var __var_5: Ref;
-if ((M_Ref_Ref[_allowances_ERC20[this]][owner_s302]) == (null)) {
+gas := (gas) - (3);
+gas := (gas) - (394);
+if ((M_Ref_Ref__allowances1[_allowances_ERC20[this]][owner_s302]) == (null)) {
 call __var_5 := FreshRefGenerator__success();
 if (revert) {
 return;
 }
-M_Ref_Ref[_allowances_ERC20[this]][owner_s302] := __var_5;
-M_Ref_int[M_Ref_Ref[_allowances_ERC20[this]][owner_s302]] := zeroRefIntArr();
+M_Ref_Ref__allowances1[_allowances_ERC20[this]][owner_s302] := __var_5;
+M_Ref_int__allowances1[M_Ref_Ref__allowances1[_allowances_ERC20[this]][owner_s302]] := zeroRefIntArr();
+sum__allowances1[M_Ref_Ref__allowances1[_allowances_ERC20[this]][owner_s302]] := 0;
 }
-assume ((M_Ref_int[M_Ref_Ref[_allowances_ERC20[this]][owner_s302]][spender_s302]) >= (0));
-__ret_0_ := M_Ref_int[M_Ref_Ref[_allowances_ERC20[this]][owner_s302]][spender_s302];
+assume ((M_Ref_int__allowances1[M_Ref_Ref__allowances1[_allowances_ERC20[this]][owner_s302]][spender_s302]) >= (0));
+__ret_0_ := M_Ref_int__allowances1[M_Ref_Ref__allowances1[_allowances_ERC20[this]][owner_s302]][spender_s302];
 return;
 }
 
 implementation approve_ERC20__fail(this: Ref, msgsender_MSG: Ref, msgvalue_MSG: int, spender_s317: Ref, amount_s317: int) returns (__ret_0_: bool)
 {
 var __var_6: bool;
+gas := (gas) - (3);
+gas := (gas) - (15);
 assume ((amount_s317) >= (0));
 call __var_6 := approve_ERC20_ERC20__fail(this, msgsender_MSG, msgvalue_MSG, spender_s317, amount_s317);
 if (revert) {
@@ -1348,6 +1744,8 @@ return;
 implementation approve_ERC20__success(this: Ref, msgsender_MSG: Ref, msgvalue_MSG: int, spender_s317: Ref, amount_s317: int) returns (__ret_0_: bool)
 {
 var __var_6: bool;
+gas := (gas) - (3);
+gas := (gas) - (15);
 assume ((amount_s317) >= (0));
 call __var_6 := approve_ERC20_ERC20__success(this, msgsender_MSG, msgvalue_MSG, spender_s317, amount_s317);
 if (revert) {
@@ -1360,6 +1758,8 @@ return;
 implementation approve_ERC20_ERC20__fail(this: Ref, msgsender_MSG: Ref, msgvalue_MSG: int, spender_s336: Ref, amount_s336: int) returns (__ret_0_: bool)
 {
 var __var_7: Ref;
+gas := (gas) - (3);
+gas := (gas) - (14);
 if ((__tmp__DType[this]) == (ERC20)) {
 call __var_7 := _msgSender_Context__fail(this, msgsender_MSG, msgvalue_MSG);
 if (revert) {
@@ -1373,6 +1773,7 @@ call _approve_ERC20__fail(this, msgsender_MSG, msgvalue_MSG, __var_7, spender_s3
 if (revert) {
 return;
 }
+gas := (gas) - (8);
 __ret_0_ := true;
 return;
 }
@@ -1380,6 +1781,8 @@ return;
 implementation approve_ERC20_ERC20__success(this: Ref, msgsender_MSG: Ref, msgvalue_MSG: int, spender_s336: Ref, amount_s336: int) returns (__ret_0_: bool)
 {
 var __var_7: Ref;
+gas := (gas) - (3);
+gas := (gas) - (14);
 if ((DType[this]) == (ERC20)) {
 call __var_7 := _msgSender_Context__success(this, msgsender_MSG, msgvalue_MSG);
 if (revert) {
@@ -1393,6 +1796,7 @@ call _approve_ERC20__success(this, msgsender_MSG, msgvalue_MSG, __var_7, spender
 if (revert) {
 return;
 }
+gas := (gas) - (8);
 __ret_0_ := true;
 return;
 }
@@ -1400,6 +1804,8 @@ return;
 implementation transferFrom_ERC20__fail(this: Ref, msgsender_MSG: Ref, msgvalue_MSG: int, sender_s354: Ref, recipient_s354: Ref, amount_s354: int) returns (__ret_0_: bool)
 {
 var __var_8: bool;
+gas := (gas) - (3);
+gas := (gas) - (18);
 assume ((amount_s354) >= (0));
 call __var_8 := transferFrom_ERC20_ERC20__fail(this, msgsender_MSG, msgvalue_MSG, sender_s354, recipient_s354, amount_s354);
 if (revert) {
@@ -1412,6 +1818,8 @@ return;
 implementation transferFrom_ERC20__success(this: Ref, msgsender_MSG: Ref, msgvalue_MSG: int, sender_s354: Ref, recipient_s354: Ref, amount_s354: int) returns (__ret_0_: bool)
 {
 var __var_8: bool;
+gas := (gas) - (3);
+gas := (gas) - (18);
 assume ((amount_s354) >= (0));
 call __var_8 := transferFrom_ERC20_ERC20__success(this, msgsender_MSG, msgvalue_MSG, sender_s354, recipient_s354, amount_s354);
 if (revert) {
@@ -1427,11 +1835,14 @@ var __var_9: Ref;
 var __var_10: int;
 var __var_11: Ref;
 var __var_12: Ref;
+gas := (gas) - (3);
+gas := (gas) - (13);
 assume ((amount_s389) >= (0));
 call _transfer_ERC20__fail(this, msgsender_MSG, msgvalue_MSG, sender_s389, recipient_s389, amount_s389);
 if (revert) {
 return;
 }
+gas := (gas) - (946);
 if ((__tmp__DType[this]) == (ERC20)) {
 call __var_9 := _msgSender_Context__fail(this, msgsender_MSG, msgvalue_MSG);
 if (revert) {
@@ -1449,17 +1860,18 @@ return;
 } else {
 assume (false);
 }
-if ((__tmp__M_Ref_Ref[__tmp___allowances_ERC20[this]][sender_s389]) == (null)) {
+if ((__tmp__M_Ref_Ref__allowances1[__tmp___allowances_ERC20[this]][sender_s389]) == (null)) {
 call __var_12 := FreshRefGenerator__fail();
 if (revert) {
 return;
 }
-__tmp__M_Ref_Ref[__tmp___allowances_ERC20[this]][sender_s389] := __var_12;
-__tmp__M_Ref_int[__tmp__M_Ref_Ref[__tmp___allowances_ERC20[this]][sender_s389]] := zeroRefIntArr();
+__tmp__M_Ref_Ref__allowances1[__tmp___allowances_ERC20[this]][sender_s389] := __var_12;
+__tmp__M_Ref_int__allowances1[__tmp__M_Ref_Ref__allowances1[__tmp___allowances_ERC20[this]][sender_s389]] := zeroRefIntArr();
+__tmp__sum__allowances1[__tmp__M_Ref_Ref__allowances1[__tmp___allowances_ERC20[this]][sender_s389]] := 0;
 }
-assume ((__tmp__M_Ref_int[__tmp__M_Ref_Ref[__tmp___allowances_ERC20[this]][sender_s389]][__var_11]) >= (0));
+assume ((__tmp__M_Ref_int__allowances1[__tmp__M_Ref_Ref__allowances1[__tmp___allowances_ERC20[this]][sender_s389]][__var_11]) >= (0));
 assume ((amount_s389) >= (0));
-call __var_10 := sub_SafeMath__fail(this, this, 0, __tmp__M_Ref_int[__tmp__M_Ref_Ref[__tmp___allowances_ERC20[this]][sender_s389]][__var_11], amount_s389);
+call __var_10 := sub_SafeMath__fail(this, this, 0, __tmp__M_Ref_int__allowances1[__tmp__M_Ref_Ref__allowances1[__tmp___allowances_ERC20[this]][sender_s389]][__var_11], amount_s389);
 if (revert) {
 return;
 }
@@ -1468,6 +1880,7 @@ call _approve_ERC20__fail(this, msgsender_MSG, msgvalue_MSG, sender_s389, __var_
 if (revert) {
 return;
 }
+gas := (gas) - (8);
 __ret_0_ := true;
 return;
 }
@@ -1478,11 +1891,14 @@ var __var_9: Ref;
 var __var_10: int;
 var __var_11: Ref;
 var __var_12: Ref;
+gas := (gas) - (3);
+gas := (gas) - (13);
 assume ((amount_s389) >= (0));
 call _transfer_ERC20__success(this, msgsender_MSG, msgvalue_MSG, sender_s389, recipient_s389, amount_s389);
 if (revert) {
 return;
 }
+gas := (gas) - (946);
 if ((DType[this]) == (ERC20)) {
 call __var_9 := _msgSender_Context__success(this, msgsender_MSG, msgvalue_MSG);
 if (revert) {
@@ -1500,17 +1916,18 @@ return;
 } else {
 assume (false);
 }
-if ((M_Ref_Ref[_allowances_ERC20[this]][sender_s389]) == (null)) {
+if ((M_Ref_Ref__allowances1[_allowances_ERC20[this]][sender_s389]) == (null)) {
 call __var_12 := FreshRefGenerator__success();
 if (revert) {
 return;
 }
-M_Ref_Ref[_allowances_ERC20[this]][sender_s389] := __var_12;
-M_Ref_int[M_Ref_Ref[_allowances_ERC20[this]][sender_s389]] := zeroRefIntArr();
+M_Ref_Ref__allowances1[_allowances_ERC20[this]][sender_s389] := __var_12;
+M_Ref_int__allowances1[M_Ref_Ref__allowances1[_allowances_ERC20[this]][sender_s389]] := zeroRefIntArr();
+sum__allowances1[M_Ref_Ref__allowances1[_allowances_ERC20[this]][sender_s389]] := 0;
 }
-assume ((M_Ref_int[M_Ref_Ref[_allowances_ERC20[this]][sender_s389]][__var_11]) >= (0));
+assume ((M_Ref_int__allowances1[M_Ref_Ref__allowances1[_allowances_ERC20[this]][sender_s389]][__var_11]) >= (0));
 assume ((amount_s389) >= (0));
-call __var_10 := sub_SafeMath__success(this, this, 0, M_Ref_int[M_Ref_Ref[_allowances_ERC20[this]][sender_s389]][__var_11], amount_s389);
+call __var_10 := sub_SafeMath__success(this, this, 0, M_Ref_int__allowances1[M_Ref_Ref__allowances1[_allowances_ERC20[this]][sender_s389]][__var_11], amount_s389);
 if (revert) {
 return;
 }
@@ -1519,6 +1936,7 @@ call _approve_ERC20__success(this, msgsender_MSG, msgvalue_MSG, sender_s389, __v
 if (revert) {
 return;
 }
+gas := (gas) - (8);
 __ret_0_ := true;
 return;
 }
@@ -1526,6 +1944,8 @@ return;
 implementation increaseAllowance_ERC20__fail(this: Ref, msgsender_MSG: Ref, msgvalue_MSG: int, spender_s404: Ref, addedValue_s404: int) returns (__ret_0_: bool)
 {
 var __var_13: bool;
+gas := (gas) - (3);
+gas := (gas) - (15);
 assume ((addedValue_s404) >= (0));
 call __var_13 := increaseAllowance_ERC20_ERC20__fail(this, msgsender_MSG, msgvalue_MSG, spender_s404, addedValue_s404);
 if (revert) {
@@ -1538,6 +1958,8 @@ return;
 implementation increaseAllowance_ERC20__success(this: Ref, msgsender_MSG: Ref, msgvalue_MSG: int, spender_s404: Ref, addedValue_s404: int) returns (__ret_0_: bool)
 {
 var __var_13: bool;
+gas := (gas) - (3);
+gas := (gas) - (15);
 assume ((addedValue_s404) >= (0));
 call __var_13 := increaseAllowance_ERC20_ERC20__success(this, msgsender_MSG, msgvalue_MSG, spender_s404, addedValue_s404);
 if (revert) {
@@ -1553,6 +1975,8 @@ var __var_14: Ref;
 var __var_15: int;
 var __var_16: Ref;
 var __var_17: Ref;
+gas := (gas) - (3);
+gas := (gas) - (940);
 if ((__tmp__DType[this]) == (ERC20)) {
 call __var_14 := _msgSender_Context__fail(this, msgsender_MSG, msgvalue_MSG);
 if (revert) {
@@ -1570,17 +1994,18 @@ return;
 } else {
 assume (false);
 }
-if ((__tmp__M_Ref_Ref[__tmp___allowances_ERC20[this]][__var_16]) == (null)) {
+if ((__tmp__M_Ref_Ref__allowances1[__tmp___allowances_ERC20[this]][__var_16]) == (null)) {
 call __var_17 := FreshRefGenerator__fail();
 if (revert) {
 return;
 }
-__tmp__M_Ref_Ref[__tmp___allowances_ERC20[this]][__var_16] := __var_17;
-__tmp__M_Ref_int[__tmp__M_Ref_Ref[__tmp___allowances_ERC20[this]][__var_16]] := zeroRefIntArr();
+__tmp__M_Ref_Ref__allowances1[__tmp___allowances_ERC20[this]][__var_16] := __var_17;
+__tmp__M_Ref_int__allowances1[__tmp__M_Ref_Ref__allowances1[__tmp___allowances_ERC20[this]][__var_16]] := zeroRefIntArr();
+__tmp__sum__allowances1[__tmp__M_Ref_Ref__allowances1[__tmp___allowances_ERC20[this]][__var_16]] := 0;
 }
-assume ((__tmp__M_Ref_int[__tmp__M_Ref_Ref[__tmp___allowances_ERC20[this]][__var_16]][spender_s431]) >= (0));
+assume ((__tmp__M_Ref_int__allowances1[__tmp__M_Ref_Ref__allowances1[__tmp___allowances_ERC20[this]][__var_16]][spender_s431]) >= (0));
 assume ((addedValue_s431) >= (0));
-call __var_15 := add_SafeMath__fail(this, this, 0, __tmp__M_Ref_int[__tmp__M_Ref_Ref[__tmp___allowances_ERC20[this]][__var_16]][spender_s431], addedValue_s431);
+call __var_15 := add_SafeMath__fail(this, this, 0, __tmp__M_Ref_int__allowances1[__tmp__M_Ref_Ref__allowances1[__tmp___allowances_ERC20[this]][__var_16]][spender_s431], addedValue_s431);
 if (revert) {
 return;
 }
@@ -1589,6 +2014,7 @@ call _approve_ERC20__fail(this, msgsender_MSG, msgvalue_MSG, __var_14, spender_s
 if (revert) {
 return;
 }
+gas := (gas) - (8);
 __ret_0_ := true;
 return;
 }
@@ -1599,6 +2025,8 @@ var __var_14: Ref;
 var __var_15: int;
 var __var_16: Ref;
 var __var_17: Ref;
+gas := (gas) - (3);
+gas := (gas) - (940);
 if ((DType[this]) == (ERC20)) {
 call __var_14 := _msgSender_Context__success(this, msgsender_MSG, msgvalue_MSG);
 if (revert) {
@@ -1616,17 +2044,18 @@ return;
 } else {
 assume (false);
 }
-if ((M_Ref_Ref[_allowances_ERC20[this]][__var_16]) == (null)) {
+if ((M_Ref_Ref__allowances1[_allowances_ERC20[this]][__var_16]) == (null)) {
 call __var_17 := FreshRefGenerator__success();
 if (revert) {
 return;
 }
-M_Ref_Ref[_allowances_ERC20[this]][__var_16] := __var_17;
-M_Ref_int[M_Ref_Ref[_allowances_ERC20[this]][__var_16]] := zeroRefIntArr();
+M_Ref_Ref__allowances1[_allowances_ERC20[this]][__var_16] := __var_17;
+M_Ref_int__allowances1[M_Ref_Ref__allowances1[_allowances_ERC20[this]][__var_16]] := zeroRefIntArr();
+sum__allowances1[M_Ref_Ref__allowances1[_allowances_ERC20[this]][__var_16]] := 0;
 }
-assume ((M_Ref_int[M_Ref_Ref[_allowances_ERC20[this]][__var_16]][spender_s431]) >= (0));
+assume ((M_Ref_int__allowances1[M_Ref_Ref__allowances1[_allowances_ERC20[this]][__var_16]][spender_s431]) >= (0));
 assume ((addedValue_s431) >= (0));
-call __var_15 := add_SafeMath__success(this, this, 0, M_Ref_int[M_Ref_Ref[_allowances_ERC20[this]][__var_16]][spender_s431], addedValue_s431);
+call __var_15 := add_SafeMath__success(this, this, 0, M_Ref_int__allowances1[M_Ref_Ref__allowances1[_allowances_ERC20[this]][__var_16]][spender_s431], addedValue_s431);
 if (revert) {
 return;
 }
@@ -1635,6 +2064,7 @@ call _approve_ERC20__success(this, msgsender_MSG, msgvalue_MSG, __var_14, spende
 if (revert) {
 return;
 }
+gas := (gas) - (8);
 __ret_0_ := true;
 return;
 }
@@ -1642,6 +2072,8 @@ return;
 implementation decreaseAllowance_ERC20__fail(this: Ref, msgsender_MSG: Ref, msgvalue_MSG: int, spender_s446: Ref, subtractedValue_s446: int) returns (__ret_0_: bool)
 {
 var __var_18: bool;
+gas := (gas) - (3);
+gas := (gas) - (15);
 assume ((subtractedValue_s446) >= (0));
 call __var_18 := decreaseAllowance_ERC20_ERC20__fail(this, msgsender_MSG, msgvalue_MSG, spender_s446, subtractedValue_s446);
 if (revert) {
@@ -1654,6 +2086,8 @@ return;
 implementation decreaseAllowance_ERC20__success(this: Ref, msgsender_MSG: Ref, msgvalue_MSG: int, spender_s446: Ref, subtractedValue_s446: int) returns (__ret_0_: bool)
 {
 var __var_18: bool;
+gas := (gas) - (3);
+gas := (gas) - (15);
 assume ((subtractedValue_s446) >= (0));
 call __var_18 := decreaseAllowance_ERC20_ERC20__success(this, msgsender_MSG, msgvalue_MSG, spender_s446, subtractedValue_s446);
 if (revert) {
@@ -1669,6 +2103,8 @@ var __var_19: Ref;
 var __var_20: int;
 var __var_21: Ref;
 var __var_22: Ref;
+gas := (gas) - (3);
+gas := (gas) - (940);
 if ((__tmp__DType[this]) == (ERC20)) {
 call __var_19 := _msgSender_Context__fail(this, msgsender_MSG, msgvalue_MSG);
 if (revert) {
@@ -1686,17 +2122,18 @@ return;
 } else {
 assume (false);
 }
-if ((__tmp__M_Ref_Ref[__tmp___allowances_ERC20[this]][__var_21]) == (null)) {
+if ((__tmp__M_Ref_Ref__allowances1[__tmp___allowances_ERC20[this]][__var_21]) == (null)) {
 call __var_22 := FreshRefGenerator__fail();
 if (revert) {
 return;
 }
-__tmp__M_Ref_Ref[__tmp___allowances_ERC20[this]][__var_21] := __var_22;
-__tmp__M_Ref_int[__tmp__M_Ref_Ref[__tmp___allowances_ERC20[this]][__var_21]] := zeroRefIntArr();
+__tmp__M_Ref_Ref__allowances1[__tmp___allowances_ERC20[this]][__var_21] := __var_22;
+__tmp__M_Ref_int__allowances1[__tmp__M_Ref_Ref__allowances1[__tmp___allowances_ERC20[this]][__var_21]] := zeroRefIntArr();
+__tmp__sum__allowances1[__tmp__M_Ref_Ref__allowances1[__tmp___allowances_ERC20[this]][__var_21]] := 0;
 }
-assume ((__tmp__M_Ref_int[__tmp__M_Ref_Ref[__tmp___allowances_ERC20[this]][__var_21]][spender_s473]) >= (0));
+assume ((__tmp__M_Ref_int__allowances1[__tmp__M_Ref_Ref__allowances1[__tmp___allowances_ERC20[this]][__var_21]][spender_s473]) >= (0));
 assume ((subtractedValue_s473) >= (0));
-call __var_20 := sub_SafeMath__fail(this, this, 0, __tmp__M_Ref_int[__tmp__M_Ref_Ref[__tmp___allowances_ERC20[this]][__var_21]][spender_s473], subtractedValue_s473);
+call __var_20 := sub_SafeMath__fail(this, this, 0, __tmp__M_Ref_int__allowances1[__tmp__M_Ref_Ref__allowances1[__tmp___allowances_ERC20[this]][__var_21]][spender_s473], subtractedValue_s473);
 if (revert) {
 return;
 }
@@ -1705,6 +2142,7 @@ call _approve_ERC20__fail(this, msgsender_MSG, msgvalue_MSG, __var_19, spender_s
 if (revert) {
 return;
 }
+gas := (gas) - (8);
 __ret_0_ := true;
 return;
 }
@@ -1715,6 +2153,8 @@ var __var_19: Ref;
 var __var_20: int;
 var __var_21: Ref;
 var __var_22: Ref;
+gas := (gas) - (3);
+gas := (gas) - (940);
 if ((DType[this]) == (ERC20)) {
 call __var_19 := _msgSender_Context__success(this, msgsender_MSG, msgvalue_MSG);
 if (revert) {
@@ -1732,17 +2172,18 @@ return;
 } else {
 assume (false);
 }
-if ((M_Ref_Ref[_allowances_ERC20[this]][__var_21]) == (null)) {
+if ((M_Ref_Ref__allowances1[_allowances_ERC20[this]][__var_21]) == (null)) {
 call __var_22 := FreshRefGenerator__success();
 if (revert) {
 return;
 }
-M_Ref_Ref[_allowances_ERC20[this]][__var_21] := __var_22;
-M_Ref_int[M_Ref_Ref[_allowances_ERC20[this]][__var_21]] := zeroRefIntArr();
+M_Ref_Ref__allowances1[_allowances_ERC20[this]][__var_21] := __var_22;
+M_Ref_int__allowances1[M_Ref_Ref__allowances1[_allowances_ERC20[this]][__var_21]] := zeroRefIntArr();
+sum__allowances1[M_Ref_Ref__allowances1[_allowances_ERC20[this]][__var_21]] := 0;
 }
-assume ((M_Ref_int[M_Ref_Ref[_allowances_ERC20[this]][__var_21]][spender_s473]) >= (0));
+assume ((M_Ref_int__allowances1[M_Ref_Ref__allowances1[_allowances_ERC20[this]][__var_21]][spender_s473]) >= (0));
 assume ((subtractedValue_s473) >= (0));
-call __var_20 := sub_SafeMath__success(this, this, 0, M_Ref_int[M_Ref_Ref[_allowances_ERC20[this]][__var_21]][spender_s473], subtractedValue_s473);
+call __var_20 := sub_SafeMath__success(this, this, 0, M_Ref_int__allowances1[M_Ref_Ref__allowances1[_allowances_ERC20[this]][__var_21]][spender_s473], subtractedValue_s473);
 if (revert) {
 return;
 }
@@ -1751,6 +2192,7 @@ call _approve_ERC20__success(this, msgsender_MSG, msgvalue_MSG, __var_19, spende
 if (revert) {
 return;
 }
+gas := (gas) - (8);
 __ret_0_ := true;
 return;
 }
@@ -1761,33 +2203,41 @@ var __var_23: Ref;
 var __var_24: Ref;
 var __var_25: int;
 var __var_26: int;
+gas := (gas) - (683);
 __var_23 := null;
 if (!((sender_s529) != (null))) {
 revert := true;
 return;
 }
+gas := (gas) - (683);
 __var_24 := null;
 if (!((recipient_s529) != (null))) {
 revert := true;
 return;
 }
-assume ((__tmp__M_Ref_int[__tmp___balances_ERC20[this]][sender_s529]) >= (0));
-assume ((__tmp__M_Ref_int[__tmp___balances_ERC20[this]][sender_s529]) >= (0));
+gas := (gas) - (20439);
+assume ((__tmp__M_Ref_int__balances0[__tmp___balances_ERC20[this]][sender_s529]) >= (0));
+assume ((__tmp__M_Ref_int__balances0[__tmp___balances_ERC20[this]][sender_s529]) >= (0));
 assume ((amount_s529) >= (0));
-call __var_25 := sub_SafeMath__fail(this, this, 0, __tmp__M_Ref_int[__tmp___balances_ERC20[this]][sender_s529], amount_s529);
+call __var_25 := sub_SafeMath__fail(this, this, 0, __tmp__M_Ref_int__balances0[__tmp___balances_ERC20[this]][sender_s529], amount_s529);
 if (revert) {
 return;
 }
-__tmp__M_Ref_int[__tmp___balances_ERC20[this]][sender_s529] := __var_25;
+__tmp__sum__balances0[__tmp___balances_ERC20[this]] := (__tmp__sum__balances0[__tmp___balances_ERC20[this]]) - (__tmp__M_Ref_int__balances0[__tmp___balances_ERC20[this]][sender_s529]);
+__tmp__M_Ref_int__balances0[__tmp___balances_ERC20[this]][sender_s529] := __var_25;
+__tmp__sum__balances0[__tmp___balances_ERC20[this]] := (__tmp__sum__balances0[__tmp___balances_ERC20[this]]) + (__tmp__M_Ref_int__balances0[__tmp___balances_ERC20[this]][sender_s529]);
 assume ((__var_25) >= (0));
-assume ((__tmp__M_Ref_int[__tmp___balances_ERC20[this]][recipient_s529]) >= (0));
-assume ((__tmp__M_Ref_int[__tmp___balances_ERC20[this]][recipient_s529]) >= (0));
+gas := (gas) - (20433);
+assume ((__tmp__M_Ref_int__balances0[__tmp___balances_ERC20[this]][recipient_s529]) >= (0));
+assume ((__tmp__M_Ref_int__balances0[__tmp___balances_ERC20[this]][recipient_s529]) >= (0));
 assume ((amount_s529) >= (0));
-call __var_26 := add_SafeMath__fail(this, this, 0, __tmp__M_Ref_int[__tmp___balances_ERC20[this]][recipient_s529], amount_s529);
+call __var_26 := add_SafeMath__fail(this, this, 0, __tmp__M_Ref_int__balances0[__tmp___balances_ERC20[this]][recipient_s529], amount_s529);
 if (revert) {
 return;
 }
-__tmp__M_Ref_int[__tmp___balances_ERC20[this]][recipient_s529] := __var_26;
+__tmp__sum__balances0[__tmp___balances_ERC20[this]] := (__tmp__sum__balances0[__tmp___balances_ERC20[this]]) - (__tmp__M_Ref_int__balances0[__tmp___balances_ERC20[this]][recipient_s529]);
+__tmp__M_Ref_int__balances0[__tmp___balances_ERC20[this]][recipient_s529] := __var_26;
+__tmp__sum__balances0[__tmp___balances_ERC20[this]] := (__tmp__sum__balances0[__tmp___balances_ERC20[this]]) + (__tmp__M_Ref_int__balances0[__tmp___balances_ERC20[this]][recipient_s529]);
 assume ((__var_26) >= (0));
 }
 
@@ -1797,33 +2247,41 @@ var __var_23: Ref;
 var __var_24: Ref;
 var __var_25: int;
 var __var_26: int;
+gas := (gas) - (683);
 __var_23 := null;
 if (!((sender_s529) != (null))) {
 revert := true;
 return;
 }
+gas := (gas) - (683);
 __var_24 := null;
 if (!((recipient_s529) != (null))) {
 revert := true;
 return;
 }
-assume ((M_Ref_int[_balances_ERC20[this]][sender_s529]) >= (0));
-assume ((M_Ref_int[_balances_ERC20[this]][sender_s529]) >= (0));
+gas := (gas) - (20439);
+assume ((M_Ref_int__balances0[_balances_ERC20[this]][sender_s529]) >= (0));
+assume ((M_Ref_int__balances0[_balances_ERC20[this]][sender_s529]) >= (0));
 assume ((amount_s529) >= (0));
-call __var_25 := sub_SafeMath__success(this, this, 0, M_Ref_int[_balances_ERC20[this]][sender_s529], amount_s529);
+call __var_25 := sub_SafeMath__success(this, this, 0, M_Ref_int__balances0[_balances_ERC20[this]][sender_s529], amount_s529);
 if (revert) {
 return;
 }
-M_Ref_int[_balances_ERC20[this]][sender_s529] := __var_25;
+sum__balances0[_balances_ERC20[this]] := (sum__balances0[_balances_ERC20[this]]) - (M_Ref_int__balances0[_balances_ERC20[this]][sender_s529]);
+M_Ref_int__balances0[_balances_ERC20[this]][sender_s529] := __var_25;
+sum__balances0[_balances_ERC20[this]] := (sum__balances0[_balances_ERC20[this]]) + (M_Ref_int__balances0[_balances_ERC20[this]][sender_s529]);
 assume ((__var_25) >= (0));
-assume ((M_Ref_int[_balances_ERC20[this]][recipient_s529]) >= (0));
-assume ((M_Ref_int[_balances_ERC20[this]][recipient_s529]) >= (0));
+gas := (gas) - (20433);
+assume ((M_Ref_int__balances0[_balances_ERC20[this]][recipient_s529]) >= (0));
+assume ((M_Ref_int__balances0[_balances_ERC20[this]][recipient_s529]) >= (0));
 assume ((amount_s529) >= (0));
-call __var_26 := add_SafeMath__success(this, this, 0, M_Ref_int[_balances_ERC20[this]][recipient_s529], amount_s529);
+call __var_26 := add_SafeMath__success(this, this, 0, M_Ref_int__balances0[_balances_ERC20[this]][recipient_s529], amount_s529);
 if (revert) {
 return;
 }
-M_Ref_int[_balances_ERC20[this]][recipient_s529] := __var_26;
+sum__balances0[_balances_ERC20[this]] := (sum__balances0[_balances_ERC20[this]]) - (M_Ref_int__balances0[_balances_ERC20[this]][recipient_s529]);
+M_Ref_int__balances0[_balances_ERC20[this]][recipient_s529] := __var_26;
+sum__balances0[_balances_ERC20[this]] := (sum__balances0[_balances_ERC20[this]]) + (M_Ref_int__balances0[_balances_ERC20[this]][recipient_s529]);
 assume ((__var_26) >= (0));
 assert {:EventEmitted "Transfer_ERC20"} (true);
 }
@@ -1865,14 +2323,16 @@ return;
 }
 __tmp___totalSupply_ERC20[this] := __var_28;
 assume ((__var_28) >= (0));
-assume ((__tmp__M_Ref_int[__tmp___balances_ERC20[this]][account_s585]) >= (0));
-assume ((__tmp__M_Ref_int[__tmp___balances_ERC20[this]][account_s585]) >= (0));
+assume ((__tmp__M_Ref_int__balances0[__tmp___balances_ERC20[this]][account_s585]) >= (0));
+assume ((__tmp__M_Ref_int__balances0[__tmp___balances_ERC20[this]][account_s585]) >= (0));
 assume ((amount_s585) >= (0));
-call __var_29 := add_SafeMath__fail(this, this, 0, __tmp__M_Ref_int[__tmp___balances_ERC20[this]][account_s585], amount_s585);
+call __var_29 := add_SafeMath__fail(this, this, 0, __tmp__M_Ref_int__balances0[__tmp___balances_ERC20[this]][account_s585], amount_s585);
 if (revert) {
 return;
 }
-__tmp__M_Ref_int[__tmp___balances_ERC20[this]][account_s585] := __var_29;
+__tmp__sum__balances0[__tmp___balances_ERC20[this]] := (__tmp__sum__balances0[__tmp___balances_ERC20[this]]) - (__tmp__M_Ref_int__balances0[__tmp___balances_ERC20[this]][account_s585]);
+__tmp__M_Ref_int__balances0[__tmp___balances_ERC20[this]][account_s585] := __var_29;
+__tmp__sum__balances0[__tmp___balances_ERC20[this]] := (__tmp__sum__balances0[__tmp___balances_ERC20[this]]) + (__tmp__M_Ref_int__balances0[__tmp___balances_ERC20[this]][account_s585]);
 assume ((__var_29) >= (0));
 }
 
@@ -1895,14 +2355,16 @@ return;
 }
 _totalSupply_ERC20[this] := __var_28;
 assume ((__var_28) >= (0));
-assume ((M_Ref_int[_balances_ERC20[this]][account_s585]) >= (0));
-assume ((M_Ref_int[_balances_ERC20[this]][account_s585]) >= (0));
+assume ((M_Ref_int__balances0[_balances_ERC20[this]][account_s585]) >= (0));
+assume ((M_Ref_int__balances0[_balances_ERC20[this]][account_s585]) >= (0));
 assume ((amount_s585) >= (0));
-call __var_29 := add_SafeMath__success(this, this, 0, M_Ref_int[_balances_ERC20[this]][account_s585], amount_s585);
+call __var_29 := add_SafeMath__success(this, this, 0, M_Ref_int__balances0[_balances_ERC20[this]][account_s585], amount_s585);
 if (revert) {
 return;
 }
-M_Ref_int[_balances_ERC20[this]][account_s585] := __var_29;
+sum__balances0[_balances_ERC20[this]] := (sum__balances0[_balances_ERC20[this]]) - (M_Ref_int__balances0[_balances_ERC20[this]][account_s585]);
+M_Ref_int__balances0[_balances_ERC20[this]][account_s585] := __var_29;
+sum__balances0[_balances_ERC20[this]] := (sum__balances0[_balances_ERC20[this]]) + (M_Ref_int__balances0[_balances_ERC20[this]][account_s585]);
 assume ((__var_29) >= (0));
 assert {:EventEmitted "Transfer_ERC20"} (true);
 }
@@ -1917,14 +2379,16 @@ if (!((account_s628) != (null))) {
 revert := true;
 return;
 }
-assume ((__tmp__M_Ref_int[__tmp___balances_ERC20[this]][account_s628]) >= (0));
-assume ((__tmp__M_Ref_int[__tmp___balances_ERC20[this]][account_s628]) >= (0));
+assume ((__tmp__M_Ref_int__balances0[__tmp___balances_ERC20[this]][account_s628]) >= (0));
+assume ((__tmp__M_Ref_int__balances0[__tmp___balances_ERC20[this]][account_s628]) >= (0));
 assume ((amount_s628) >= (0));
-call __var_31 := sub_SafeMath__fail(this, this, 0, __tmp__M_Ref_int[__tmp___balances_ERC20[this]][account_s628], amount_s628);
+call __var_31 := sub_SafeMath__fail(this, this, 0, __tmp__M_Ref_int__balances0[__tmp___balances_ERC20[this]][account_s628], amount_s628);
 if (revert) {
 return;
 }
-__tmp__M_Ref_int[__tmp___balances_ERC20[this]][account_s628] := __var_31;
+__tmp__sum__balances0[__tmp___balances_ERC20[this]] := (__tmp__sum__balances0[__tmp___balances_ERC20[this]]) - (__tmp__M_Ref_int__balances0[__tmp___balances_ERC20[this]][account_s628]);
+__tmp__M_Ref_int__balances0[__tmp___balances_ERC20[this]][account_s628] := __var_31;
+__tmp__sum__balances0[__tmp___balances_ERC20[this]] := (__tmp__sum__balances0[__tmp___balances_ERC20[this]]) + (__tmp__M_Ref_int__balances0[__tmp___balances_ERC20[this]][account_s628]);
 assume ((__var_31) >= (0));
 assume ((__tmp___totalSupply_ERC20[this]) >= (0));
 assume ((__tmp___totalSupply_ERC20[this]) >= (0));
@@ -1947,14 +2411,16 @@ if (!((account_s628) != (null))) {
 revert := true;
 return;
 }
-assume ((M_Ref_int[_balances_ERC20[this]][account_s628]) >= (0));
-assume ((M_Ref_int[_balances_ERC20[this]][account_s628]) >= (0));
+assume ((M_Ref_int__balances0[_balances_ERC20[this]][account_s628]) >= (0));
+assume ((M_Ref_int__balances0[_balances_ERC20[this]][account_s628]) >= (0));
 assume ((amount_s628) >= (0));
-call __var_31 := sub_SafeMath__success(this, this, 0, M_Ref_int[_balances_ERC20[this]][account_s628], amount_s628);
+call __var_31 := sub_SafeMath__success(this, this, 0, M_Ref_int__balances0[_balances_ERC20[this]][account_s628], amount_s628);
 if (revert) {
 return;
 }
-M_Ref_int[_balances_ERC20[this]][account_s628] := __var_31;
+sum__balances0[_balances_ERC20[this]] := (sum__balances0[_balances_ERC20[this]]) - (M_Ref_int__balances0[_balances_ERC20[this]][account_s628]);
+M_Ref_int__balances0[_balances_ERC20[this]][account_s628] := __var_31;
+sum__balances0[_balances_ERC20[this]] := (sum__balances0[_balances_ERC20[this]]) + (M_Ref_int__balances0[_balances_ERC20[this]][account_s628]);
 assume ((__var_31) >= (0));
 assume ((_totalSupply_ERC20[this]) >= (0));
 assume ((_totalSupply_ERC20[this]) >= (0));
@@ -1973,27 +2439,33 @@ implementation _approve_ERC20__fail(this: Ref, msgsender_MSG: Ref, msgvalue_MSG:
 var __var_33: Ref;
 var __var_34: Ref;
 var __var_35: Ref;
+gas := (gas) - (683);
 __var_33 := null;
 if (!((owner_s670) != (null))) {
 revert := true;
 return;
 }
+gas := (gas) - (683);
 __var_34 := null;
 if (!((spender_s670) != (null))) {
 revert := true;
 return;
 }
-if ((__tmp__M_Ref_Ref[__tmp___allowances_ERC20[this]][owner_s670]) == (null)) {
+gas := (gas) - (20200);
+if ((__tmp__M_Ref_Ref__allowances1[__tmp___allowances_ERC20[this]][owner_s670]) == (null)) {
 call __var_35 := FreshRefGenerator__fail();
 if (revert) {
 return;
 }
-__tmp__M_Ref_Ref[__tmp___allowances_ERC20[this]][owner_s670] := __var_35;
-__tmp__M_Ref_int[__tmp__M_Ref_Ref[__tmp___allowances_ERC20[this]][owner_s670]] := zeroRefIntArr();
+__tmp__M_Ref_Ref__allowances1[__tmp___allowances_ERC20[this]][owner_s670] := __var_35;
+__tmp__M_Ref_int__allowances1[__tmp__M_Ref_Ref__allowances1[__tmp___allowances_ERC20[this]][owner_s670]] := zeroRefIntArr();
+__tmp__sum__allowances1[__tmp__M_Ref_Ref__allowances1[__tmp___allowances_ERC20[this]][owner_s670]] := 0;
 }
-assume ((__tmp__M_Ref_int[__tmp__M_Ref_Ref[__tmp___allowances_ERC20[this]][owner_s670]][spender_s670]) >= (0));
+assume ((__tmp__M_Ref_int__allowances1[__tmp__M_Ref_Ref__allowances1[__tmp___allowances_ERC20[this]][owner_s670]][spender_s670]) >= (0));
 assume ((amount_s670) >= (0));
-__tmp__M_Ref_int[__tmp__M_Ref_Ref[__tmp___allowances_ERC20[this]][owner_s670]][spender_s670] := amount_s670;
+__tmp__sum__allowances1[__tmp__M_Ref_Ref__allowances1[__tmp___allowances_ERC20[this]][owner_s670]] := (__tmp__sum__allowances1[__tmp__M_Ref_Ref__allowances1[__tmp___allowances_ERC20[this]][owner_s670]]) - (__tmp__M_Ref_int__allowances1[__tmp__M_Ref_Ref__allowances1[__tmp___allowances_ERC20[this]][owner_s670]][spender_s670]);
+__tmp__M_Ref_int__allowances1[__tmp__M_Ref_Ref__allowances1[__tmp___allowances_ERC20[this]][owner_s670]][spender_s670] := amount_s670;
+__tmp__sum__allowances1[__tmp__M_Ref_Ref__allowances1[__tmp___allowances_ERC20[this]][owner_s670]] := (__tmp__sum__allowances1[__tmp__M_Ref_Ref__allowances1[__tmp___allowances_ERC20[this]][owner_s670]]) + (__tmp__M_Ref_int__allowances1[__tmp__M_Ref_Ref__allowances1[__tmp___allowances_ERC20[this]][owner_s670]][spender_s670]);
 }
 
 implementation _approve_ERC20__success(this: Ref, msgsender_MSG: Ref, msgvalue_MSG: int, owner_s670: Ref, spender_s670: Ref, amount_s670: int)
@@ -2001,27 +2473,33 @@ implementation _approve_ERC20__success(this: Ref, msgsender_MSG: Ref, msgvalue_M
 var __var_33: Ref;
 var __var_34: Ref;
 var __var_35: Ref;
+gas := (gas) - (683);
 __var_33 := null;
 if (!((owner_s670) != (null))) {
 revert := true;
 return;
 }
+gas := (gas) - (683);
 __var_34 := null;
 if (!((spender_s670) != (null))) {
 revert := true;
 return;
 }
-if ((M_Ref_Ref[_allowances_ERC20[this]][owner_s670]) == (null)) {
+gas := (gas) - (20200);
+if ((M_Ref_Ref__allowances1[_allowances_ERC20[this]][owner_s670]) == (null)) {
 call __var_35 := FreshRefGenerator__success();
 if (revert) {
 return;
 }
-M_Ref_Ref[_allowances_ERC20[this]][owner_s670] := __var_35;
-M_Ref_int[M_Ref_Ref[_allowances_ERC20[this]][owner_s670]] := zeroRefIntArr();
+M_Ref_Ref__allowances1[_allowances_ERC20[this]][owner_s670] := __var_35;
+M_Ref_int__allowances1[M_Ref_Ref__allowances1[_allowances_ERC20[this]][owner_s670]] := zeroRefIntArr();
+sum__allowances1[M_Ref_Ref__allowances1[_allowances_ERC20[this]][owner_s670]] := 0;
 }
-assume ((M_Ref_int[M_Ref_Ref[_allowances_ERC20[this]][owner_s670]][spender_s670]) >= (0));
+assume ((M_Ref_int__allowances1[M_Ref_Ref__allowances1[_allowances_ERC20[this]][owner_s670]][spender_s670]) >= (0));
 assume ((amount_s670) >= (0));
-M_Ref_int[M_Ref_Ref[_allowances_ERC20[this]][owner_s670]][spender_s670] := amount_s670;
+sum__allowances1[M_Ref_Ref__allowances1[_allowances_ERC20[this]][owner_s670]] := (sum__allowances1[M_Ref_Ref__allowances1[_allowances_ERC20[this]][owner_s670]]) - (M_Ref_int__allowances1[M_Ref_Ref__allowances1[_allowances_ERC20[this]][owner_s670]][spender_s670]);
+M_Ref_int__allowances1[M_Ref_Ref__allowances1[_allowances_ERC20[this]][owner_s670]][spender_s670] := amount_s670;
+sum__allowances1[M_Ref_Ref__allowances1[_allowances_ERC20[this]][owner_s670]] := (sum__allowances1[M_Ref_Ref__allowances1[_allowances_ERC20[this]][owner_s670]]) + (M_Ref_int__allowances1[M_Ref_Ref__allowances1[_allowances_ERC20[this]][owner_s670]][spender_s670]);
 assert {:EventEmitted "Approval_ERC20"} (true);
 }
 
@@ -2053,17 +2531,18 @@ return;
 } else {
 assume (false);
 }
-if ((__tmp__M_Ref_Ref[__tmp___allowances_ERC20[this]][account_s698]) == (null)) {
+if ((__tmp__M_Ref_Ref__allowances1[__tmp___allowances_ERC20[this]][account_s698]) == (null)) {
 call __var_39 := FreshRefGenerator__fail();
 if (revert) {
 return;
 }
-__tmp__M_Ref_Ref[__tmp___allowances_ERC20[this]][account_s698] := __var_39;
-__tmp__M_Ref_int[__tmp__M_Ref_Ref[__tmp___allowances_ERC20[this]][account_s698]] := zeroRefIntArr();
+__tmp__M_Ref_Ref__allowances1[__tmp___allowances_ERC20[this]][account_s698] := __var_39;
+__tmp__M_Ref_int__allowances1[__tmp__M_Ref_Ref__allowances1[__tmp___allowances_ERC20[this]][account_s698]] := zeroRefIntArr();
+__tmp__sum__allowances1[__tmp__M_Ref_Ref__allowances1[__tmp___allowances_ERC20[this]][account_s698]] := 0;
 }
-assume ((__tmp__M_Ref_int[__tmp__M_Ref_Ref[__tmp___allowances_ERC20[this]][account_s698]][__var_38]) >= (0));
+assume ((__tmp__M_Ref_int__allowances1[__tmp__M_Ref_Ref__allowances1[__tmp___allowances_ERC20[this]][account_s698]][__var_38]) >= (0));
 assume ((amount_s698) >= (0));
-call __var_37 := sub_SafeMath__fail(this, this, 0, __tmp__M_Ref_int[__tmp__M_Ref_Ref[__tmp___allowances_ERC20[this]][account_s698]][__var_38], amount_s698);
+call __var_37 := sub_SafeMath__fail(this, this, 0, __tmp__M_Ref_int__allowances1[__tmp__M_Ref_Ref__allowances1[__tmp___allowances_ERC20[this]][account_s698]][__var_38], amount_s698);
 if (revert) {
 return;
 }
@@ -2102,17 +2581,18 @@ return;
 } else {
 assume (false);
 }
-if ((M_Ref_Ref[_allowances_ERC20[this]][account_s698]) == (null)) {
+if ((M_Ref_Ref__allowances1[_allowances_ERC20[this]][account_s698]) == (null)) {
 call __var_39 := FreshRefGenerator__success();
 if (revert) {
 return;
 }
-M_Ref_Ref[_allowances_ERC20[this]][account_s698] := __var_39;
-M_Ref_int[M_Ref_Ref[_allowances_ERC20[this]][account_s698]] := zeroRefIntArr();
+M_Ref_Ref__allowances1[_allowances_ERC20[this]][account_s698] := __var_39;
+M_Ref_int__allowances1[M_Ref_Ref__allowances1[_allowances_ERC20[this]][account_s698]] := zeroRefIntArr();
+sum__allowances1[M_Ref_Ref__allowances1[_allowances_ERC20[this]][account_s698]] := 0;
 }
-assume ((M_Ref_int[M_Ref_Ref[_allowances_ERC20[this]][account_s698]][__var_38]) >= (0));
+assume ((M_Ref_int__allowances1[M_Ref_Ref__allowances1[_allowances_ERC20[this]][account_s698]][__var_38]) >= (0));
 assume ((amount_s698) >= (0));
-call __var_37 := sub_SafeMath__success(this, this, 0, M_Ref_int[M_Ref_Ref[_allowances_ERC20[this]][account_s698]][__var_38], amount_s698);
+call __var_37 := sub_SafeMath__success(this, this, 0, M_Ref_int__allowances1[M_Ref_Ref__allowances1[_allowances_ERC20[this]][account_s698]][__var_38], amount_s698);
 if (revert) {
 return;
 }
@@ -2188,53 +2668,86 @@ assume ((__tmp__Balance[from]) >= (amount));
 __tmp__Balance[from] := (__tmp__Balance[from]) - (amount);
 __tmp__Balance[to] := (__tmp__Balance[to]) + (amount);
 // ---- Logic for payable function END 
+if ((choice) == (0)) {
+revert := true;
+return;
+}
+if ((gas) < (21000)) {
+return;
+}
+if ((__tmp__DType[from]) == (ERC20)) {
 if ((choice) == (8)) {
 gas := (gas) - (21000);
+if ((gas) >= (0)) {
+assume ((msgvalue_MSG) == (0));
 call __ret_0_totalSupply := totalSupply_ERC20__fail(from, to, msgvalue_MSG);
 if (revert) {
 return;
 }
+}
 } else if ((choice) == (7)) {
 gas := (gas) - (21000);
+if ((gas) >= (0)) {
+assume ((msgvalue_MSG) == (0));
 call __ret_0_balanceOf := balanceOf_ERC20__fail(from, to, msgvalue_MSG, account_s252);
 if (revert) {
 return;
 }
+}
 } else if ((choice) == (6)) {
 gas := (gas) - (21000);
+if ((gas) >= (0)) {
+assume ((msgvalue_MSG) == (0));
 call __ret_0_transfer := transfer_ERC20__fail(from, to, msgvalue_MSG, recipient_s267, amount_s267);
 if (revert) {
 return;
 }
+}
 } else if ((choice) == (5)) {
 gas := (gas) - (21000);
+if ((gas) >= (0)) {
+assume ((msgvalue_MSG) == (0));
 call __ret_0_allowance := allowance_ERC20__fail(from, to, msgvalue_MSG, owner_s302, spender_s302);
 if (revert) {
 return;
 }
+}
 } else if ((choice) == (4)) {
 gas := (gas) - (21000);
+if ((gas) >= (0)) {
+assume ((msgvalue_MSG) == (0));
 call __ret_0_approve := approve_ERC20__fail(from, to, msgvalue_MSG, spender_s317, amount_s317);
 if (revert) {
 return;
 }
+}
 } else if ((choice) == (3)) {
 gas := (gas) - (21000);
+if ((gas) >= (0)) {
+assume ((msgvalue_MSG) == (0));
 call __ret_0_transferFrom := transferFrom_ERC20__fail(from, to, msgvalue_MSG, sender_s354, recipient_s354, amount_s354);
 if (revert) {
 return;
 }
+}
 } else if ((choice) == (2)) {
 gas := (gas) - (21000);
+if ((gas) >= (0)) {
+assume ((msgvalue_MSG) == (0));
 call __ret_0_increaseAllowance := increaseAllowance_ERC20__fail(from, to, msgvalue_MSG, spender_s404, addedValue_s404);
 if (revert) {
 return;
 }
+}
 } else if ((choice) == (1)) {
 gas := (gas) - (21000);
+if ((gas) >= (0)) {
+assume ((msgvalue_MSG) == (0));
 call __ret_0_decreaseAllowance := decreaseAllowance_ERC20__fail(from, to, msgvalue_MSG, spender_s446, subtractedValue_s446);
 if (revert) {
 return;
+}
+}
 }
 }
 }
@@ -2272,53 +2785,86 @@ assume ((Balance[from]) >= (amount));
 Balance[from] := (Balance[from]) - (amount);
 Balance[to] := (Balance[to]) + (amount);
 // ---- Logic for payable function END 
+if ((choice) == (0)) {
+revert := true;
+return;
+}
+if ((gas) < (21000)) {
+return;
+}
+if ((DType[from]) == (ERC20)) {
 if ((choice) == (8)) {
 gas := (gas) - (21000);
+if ((gas) >= (0)) {
+assume ((msgvalue_MSG) == (0));
 call __ret_0_totalSupply := totalSupply_ERC20__success(from, to, msgvalue_MSG);
 if (revert) {
 return;
 }
+}
 } else if ((choice) == (7)) {
 gas := (gas) - (21000);
+if ((gas) >= (0)) {
+assume ((msgvalue_MSG) == (0));
 call __ret_0_balanceOf := balanceOf_ERC20__success(from, to, msgvalue_MSG, account_s252);
 if (revert) {
 return;
 }
+}
 } else if ((choice) == (6)) {
 gas := (gas) - (21000);
+if ((gas) >= (0)) {
+assume ((msgvalue_MSG) == (0));
 call __ret_0_transfer := transfer_ERC20__success(from, to, msgvalue_MSG, recipient_s267, amount_s267);
 if (revert) {
 return;
 }
+}
 } else if ((choice) == (5)) {
 gas := (gas) - (21000);
+if ((gas) >= (0)) {
+assume ((msgvalue_MSG) == (0));
 call __ret_0_allowance := allowance_ERC20__success(from, to, msgvalue_MSG, owner_s302, spender_s302);
 if (revert) {
 return;
 }
+}
 } else if ((choice) == (4)) {
 gas := (gas) - (21000);
+if ((gas) >= (0)) {
+assume ((msgvalue_MSG) == (0));
 call __ret_0_approve := approve_ERC20__success(from, to, msgvalue_MSG, spender_s317, amount_s317);
 if (revert) {
 return;
 }
+}
 } else if ((choice) == (3)) {
 gas := (gas) - (21000);
+if ((gas) >= (0)) {
+assume ((msgvalue_MSG) == (0));
 call __ret_0_transferFrom := transferFrom_ERC20__success(from, to, msgvalue_MSG, sender_s354, recipient_s354, amount_s354);
 if (revert) {
 return;
 }
+}
 } else if ((choice) == (2)) {
 gas := (gas) - (21000);
+if ((gas) >= (0)) {
+assume ((msgvalue_MSG) == (0));
 call __ret_0_increaseAllowance := increaseAllowance_ERC20__success(from, to, msgvalue_MSG, spender_s404, addedValue_s404);
 if (revert) {
 return;
 }
+}
 } else if ((choice) == (1)) {
 gas := (gas) - (21000);
+if ((gas) >= (0)) {
+assume ((msgvalue_MSG) == (0));
 call __ret_0_decreaseAllowance := decreaseAllowance_ERC20__success(from, to, msgvalue_MSG, spender_s446, subtractedValue_s446);
 if (revert) {
 return;
+}
+}
 }
 }
 }
@@ -2330,9 +2876,13 @@ var __snap___tmp__Balance: [Ref]int;
 var __snap___tmp__DType: [Ref]ContractName;
 var __snap___tmp__Alloc: [Ref]bool;
 var __snap___tmp__balance_ADDR: [Ref]int;
-var __snap___tmp__M_Ref_int: [Ref][Ref]int;
-var __snap___tmp__M_Ref_Ref: [Ref][Ref]Ref;
+var __snap___tmp__M_Ref_int__balances0: [Ref][Ref]int;
+var __snap___tmp__sum__balances0: [Ref]int;
+var __snap___tmp__M_Ref_int__allowances1: [Ref][Ref]int;
+var __snap___tmp__M_Ref_Ref__allowances1: [Ref][Ref]Ref;
+var __snap___tmp__sum__allowances1: [Ref]int;
 var __snap___tmp__Length: [Ref]int;
+var __snap___tmp__now: int;
 var __snap___tmp___balances_ERC20: [Ref]Ref;
 var __snap___tmp___allowances_ERC20: [Ref]Ref;
 var __snap___tmp___totalSupply_ERC20: [Ref]int;
@@ -2342,9 +2892,13 @@ __snap___tmp__Balance := __tmp__Balance;
 __snap___tmp__DType := __tmp__DType;
 __snap___tmp__Alloc := __tmp__Alloc;
 __snap___tmp__balance_ADDR := __tmp__balance_ADDR;
-__snap___tmp__M_Ref_int := __tmp__M_Ref_int;
-__snap___tmp__M_Ref_Ref := __tmp__M_Ref_Ref;
+__snap___tmp__M_Ref_int__balances0 := __tmp__M_Ref_int__balances0;
+__snap___tmp__sum__balances0 := __tmp__sum__balances0;
+__snap___tmp__M_Ref_int__allowances1 := __tmp__M_Ref_int__allowances1;
+__snap___tmp__M_Ref_Ref__allowances1 := __tmp__M_Ref_Ref__allowances1;
+__snap___tmp__sum__allowances1 := __tmp__sum__allowances1;
 __snap___tmp__Length := __tmp__Length;
+__snap___tmp__now := __tmp__now;
 __snap___tmp___balances_ERC20 := __tmp___balances_ERC20;
 __snap___tmp___allowances_ERC20 := __tmp___allowances_ERC20;
 __snap___tmp___totalSupply_ERC20 := __tmp___totalSupply_ERC20;
@@ -2357,9 +2911,13 @@ __tmp__Balance := __snap___tmp__Balance;
 __tmp__DType := __snap___tmp__DType;
 __tmp__Alloc := __snap___tmp__Alloc;
 __tmp__balance_ADDR := __snap___tmp__balance_ADDR;
-__tmp__M_Ref_int := __snap___tmp__M_Ref_int;
-__tmp__M_Ref_Ref := __snap___tmp__M_Ref_Ref;
+__tmp__M_Ref_int__balances0 := __snap___tmp__M_Ref_int__balances0;
+__tmp__sum__balances0 := __snap___tmp__sum__balances0;
+__tmp__M_Ref_int__allowances1 := __snap___tmp__M_Ref_int__allowances1;
+__tmp__M_Ref_Ref__allowances1 := __snap___tmp__M_Ref_Ref__allowances1;
+__tmp__sum__allowances1 := __snap___tmp__sum__allowances1;
 __tmp__Length := __snap___tmp__Length;
+__tmp__now := __snap___tmp__now;
 __tmp___balances_ERC20 := __snap___tmp___balances_ERC20;
 __tmp___allowances_ERC20 := __snap___tmp___allowances_ERC20;
 __tmp___totalSupply_ERC20 := __snap___tmp___totalSupply_ERC20;
@@ -2384,9 +2942,13 @@ __tmp__Balance := Balance;
 __tmp__DType := DType;
 __tmp__Alloc := Alloc;
 __tmp__balance_ADDR := balance_ADDR;
-__tmp__M_Ref_int := M_Ref_int;
-__tmp__M_Ref_Ref := M_Ref_Ref;
+__tmp__M_Ref_int__balances0 := M_Ref_int__balances0;
+__tmp__sum__balances0 := sum__balances0;
+__tmp__M_Ref_int__allowances1 := M_Ref_int__allowances1;
+__tmp__M_Ref_Ref__allowances1 := M_Ref_Ref__allowances1;
+__tmp__sum__allowances1 := sum__allowances1;
 __tmp__Length := Length;
+__tmp__now := now;
 __tmp___balances_ERC20 := _balances_ERC20;
 __tmp___allowances_ERC20 := _allowances_ERC20;
 __tmp___totalSupply_ERC20 := _totalSupply_ERC20;
@@ -2407,165 +2969,27 @@ assume ((!(revert)) && ((gas) >= (0)));
 }
 }
 
-implementation BoogieEntry_Context()
-{
-var this: Ref;
-var msgsender_MSG: Ref;
-var msgvalue_MSG: int;
-var choice: int;
-assume (((DType[this]) == (Context)) || ((DType[this]) == (ERC20)));
-gas := (gas) - (53000);
-call Context_Context(this, msgsender_MSG, msgvalue_MSG);
-assume ((!(revert)) && ((gas) >= (0)));
-while (true)
-{
-havoc msgsender_MSG;
-havoc msgvalue_MSG;
-havoc choice;
-havoc gas;
-assume (((gas) > (4000000)) && ((gas) <= (8000000)));
-}
-}
-
-implementation BoogieEntry_SafeMath()
-{
-var this: Ref;
-var msgsender_MSG: Ref;
-var msgvalue_MSG: int;
-var choice: int;
-assume ((DType[this]) == (SafeMath));
-gas := (gas) - (53000);
-call SafeMath_SafeMath__success(this, msgsender_MSG, msgvalue_MSG);
-assume ((!(revert)) && ((gas) >= (0)));
-while (true)
-{
-havoc msgsender_MSG;
-havoc msgvalue_MSG;
-havoc choice;
-havoc gas;
-assume (((gas) > (4000000)) && ((gas) <= (8000000)));
-}
-}
-
-implementation BoogieEntry_IERC20()
-{
-var this: Ref;
-var msgsender_MSG: Ref;
-var msgvalue_MSG: int;
-var choice: int;
-assume (((DType[this]) == (IERC20)) || ((DType[this]) == (ERC20)));
-gas := (gas) - (53000);
-call IERC20_IERC20__success(this, msgsender_MSG, msgvalue_MSG);
-assume ((!(revert)) && ((gas) >= (0)));
-while (true)
-{
-havoc msgsender_MSG;
-havoc msgvalue_MSG;
-havoc choice;
-havoc gas;
-assume (((gas) > (4000000)) && ((gas) <= (8000000)));
-}
-}
-
-implementation BoogieEntry_ERC20()
-{
-var this: Ref;
-var msgsender_MSG: Ref;
-var msgvalue_MSG: int;
-var choice: int;
-var __ret_0_totalSupply: int;
-var account_s252: Ref;
-var __ret_0_balanceOf: int;
-var recipient_s267: Ref;
-var amount_s267: int;
-var __ret_0_transfer: bool;
-var owner_s302: Ref;
-var spender_s302: Ref;
-var __ret_0_allowance: int;
-var spender_s317: Ref;
-var amount_s317: int;
-var __ret_0_approve: bool;
-var sender_s354: Ref;
-var recipient_s354: Ref;
-var amount_s354: int;
-var __ret_0_transferFrom: bool;
-var spender_s404: Ref;
-var addedValue_s404: int;
-var __ret_0_increaseAllowance: bool;
-var spender_s446: Ref;
-var subtractedValue_s446: int;
-var __ret_0_decreaseAllowance: bool;
-assume ((DType[this]) == (ERC20));
-gas := (gas) - (53000);
-call ERC20_ERC20__success(this, msgsender_MSG, msgvalue_MSG);
-assume ((!(revert)) && ((gas) >= (0)));
-while (true)
-{
-havoc msgsender_MSG;
-havoc msgvalue_MSG;
-havoc choice;
-havoc __ret_0_totalSupply;
-havoc account_s252;
-havoc __ret_0_balanceOf;
-havoc recipient_s267;
-havoc amount_s267;
-havoc __ret_0_transfer;
-havoc owner_s302;
-havoc spender_s302;
-havoc __ret_0_allowance;
-havoc spender_s317;
-havoc amount_s317;
-havoc __ret_0_approve;
-havoc sender_s354;
-havoc recipient_s354;
-havoc amount_s354;
-havoc __ret_0_transferFrom;
-havoc spender_s404;
-havoc addedValue_s404;
-havoc __ret_0_increaseAllowance;
-havoc spender_s446;
-havoc subtractedValue_s446;
-havoc __ret_0_decreaseAllowance;
-havoc gas;
-assume (((gas) > (4000000)) && ((gas) <= (8000000)));
-if ((choice) == (8)) {
-gas := (gas) - (21000);
-call __ret_0_totalSupply := totalSupply_ERC20(this, msgsender_MSG, msgvalue_MSG);
-} else if ((choice) == (7)) {
-gas := (gas) - (21000);
-call __ret_0_balanceOf := balanceOf_ERC20(this, msgsender_MSG, msgvalue_MSG, account_s252);
-} else if ((choice) == (6)) {
-gas := (gas) - (21000);
-call __ret_0_transfer := transfer_ERC20(this, msgsender_MSG, msgvalue_MSG, recipient_s267, amount_s267);
-} else if ((choice) == (5)) {
-gas := (gas) - (21000);
-call __ret_0_allowance := allowance_ERC20(this, msgsender_MSG, msgvalue_MSG, owner_s302, spender_s302);
-} else if ((choice) == (4)) {
-gas := (gas) - (21000);
-call __ret_0_approve := approve_ERC20(this, msgsender_MSG, msgvalue_MSG, spender_s317, amount_s317);
-} else if ((choice) == (3)) {
-gas := (gas) - (21000);
-call __ret_0_transferFrom := transferFrom_ERC20(this, msgsender_MSG, msgvalue_MSG, sender_s354, recipient_s354, amount_s354);
-} else if ((choice) == (2)) {
-gas := (gas) - (21000);
-call __ret_0_increaseAllowance := increaseAllowance_ERC20(this, msgsender_MSG, msgvalue_MSG, spender_s404, addedValue_s404);
-} else if ((choice) == (1)) {
-gas := (gas) - (21000);
-call __ret_0_decreaseAllowance := decreaseAllowance_ERC20(this, msgsender_MSG, msgvalue_MSG, spender_s446, subtractedValue_s446);
-}
-}
-}
-
 implementation CorralChoice_Context(this: Ref)
 {
 var msgsender_MSG: Ref;
 var msgvalue_MSG: int;
 var choice: int;
+var tmpNow: int;
 havoc msgsender_MSG;
 havoc msgvalue_MSG;
 havoc choice;
+havoc tmpNow;
 havoc gas;
 assume (((gas) > (4000000)) && ((gas) <= (8000000)));
+tmpNow := now;
+havoc now;
+assume ((now) > (tmpNow));
+assume ((msgsender_MSG) != (null));
+assume ((DType[msgsender_MSG]) != (Context));
+assume ((DType[msgsender_MSG]) != (SafeMath));
+assume ((DType[msgsender_MSG]) != (IERC20));
+assume ((DType[msgsender_MSG]) != (ERC20));
+Alloc[msgsender_MSG] := true;
 }
 
 implementation CorralEntry_Context()
@@ -2573,6 +2997,9 @@ implementation CorralEntry_Context()
 var this: Ref;
 var msgsender_MSG: Ref;
 var msgvalue_MSG: int;
+assume ((null) == (0));
+call this := FreshRefGenerator__success();
+assume ((now) >= (0));
 assume (((DType[this]) == (Context)) || ((DType[this]) == (ERC20)));
 gas := (gas) - (53000);
 call Context_Context(this, msgsender_MSG, msgvalue_MSG);
@@ -2588,11 +3015,22 @@ implementation CorralChoice_SafeMath(this: Ref)
 var msgsender_MSG: Ref;
 var msgvalue_MSG: int;
 var choice: int;
+var tmpNow: int;
 havoc msgsender_MSG;
 havoc msgvalue_MSG;
 havoc choice;
+havoc tmpNow;
 havoc gas;
 assume (((gas) > (4000000)) && ((gas) <= (8000000)));
+tmpNow := now;
+havoc now;
+assume ((now) > (tmpNow));
+assume ((msgsender_MSG) != (null));
+assume ((DType[msgsender_MSG]) != (Context));
+assume ((DType[msgsender_MSG]) != (SafeMath));
+assume ((DType[msgsender_MSG]) != (IERC20));
+assume ((DType[msgsender_MSG]) != (ERC20));
+Alloc[msgsender_MSG] := true;
 }
 
 implementation CorralEntry_SafeMath()
@@ -2600,6 +3038,9 @@ implementation CorralEntry_SafeMath()
 var this: Ref;
 var msgsender_MSG: Ref;
 var msgvalue_MSG: int;
+assume ((null) == (0));
+call this := FreshRefGenerator__success();
+assume ((now) >= (0));
 assume ((DType[this]) == (SafeMath));
 gas := (gas) - (53000);
 call SafeMath_SafeMath__success(this, msgsender_MSG, msgvalue_MSG);
@@ -2615,11 +3056,22 @@ implementation CorralChoice_IERC20(this: Ref)
 var msgsender_MSG: Ref;
 var msgvalue_MSG: int;
 var choice: int;
+var tmpNow: int;
 havoc msgsender_MSG;
 havoc msgvalue_MSG;
 havoc choice;
+havoc tmpNow;
 havoc gas;
 assume (((gas) > (4000000)) && ((gas) <= (8000000)));
+tmpNow := now;
+havoc now;
+assume ((now) > (tmpNow));
+assume ((msgsender_MSG) != (null));
+assume ((DType[msgsender_MSG]) != (Context));
+assume ((DType[msgsender_MSG]) != (SafeMath));
+assume ((DType[msgsender_MSG]) != (IERC20));
+assume ((DType[msgsender_MSG]) != (ERC20));
+Alloc[msgsender_MSG] := true;
 }
 
 implementation CorralEntry_IERC20()
@@ -2627,6 +3079,9 @@ implementation CorralEntry_IERC20()
 var this: Ref;
 var msgsender_MSG: Ref;
 var msgvalue_MSG: int;
+assume ((null) == (0));
+call this := FreshRefGenerator__success();
+assume ((now) >= (0));
 assume (((DType[this]) == (IERC20)) || ((DType[this]) == (ERC20)));
 gas := (gas) - (53000);
 call IERC20_IERC20__success(this, msgsender_MSG, msgvalue_MSG);
@@ -2664,6 +3119,7 @@ var __ret_0_increaseAllowance: bool;
 var spender_s446: Ref;
 var subtractedValue_s446: int;
 var __ret_0_decreaseAllowance: bool;
+var tmpNow: int;
 havoc msgsender_MSG;
 havoc msgvalue_MSG;
 havoc choice;
@@ -2689,40 +3145,77 @@ havoc __ret_0_increaseAllowance;
 havoc spender_s446;
 havoc subtractedValue_s446;
 havoc __ret_0_decreaseAllowance;
+havoc tmpNow;
 havoc gas;
 assume (((gas) > (4000000)) && ((gas) <= (8000000)));
+tmpNow := now;
+havoc now;
+assume ((now) > (tmpNow));
+assume ((msgsender_MSG) != (null));
+assume ((DType[msgsender_MSG]) != (Context));
+assume ((DType[msgsender_MSG]) != (SafeMath));
+assume ((DType[msgsender_MSG]) != (IERC20));
+assume ((DType[msgsender_MSG]) != (ERC20));
+Alloc[msgsender_MSG] := true;
 if ((choice) == (8)) {
 gas := (gas) - (21000);
+if ((gas) >= (0)) {
+assume ((msgvalue_MSG) == (0));
 call __ret_0_totalSupply := totalSupply_ERC20(this, msgsender_MSG, msgvalue_MSG);
+}
 } else if ((choice) == (7)) {
 gas := (gas) - (21000);
+if ((gas) >= (0)) {
+assume ((msgvalue_MSG) == (0));
 call __ret_0_balanceOf := balanceOf_ERC20(this, msgsender_MSG, msgvalue_MSG, account_s252);
+}
 } else if ((choice) == (6)) {
 gas := (gas) - (21000);
+if ((gas) >= (0)) {
+assume ((msgvalue_MSG) == (0));
 call __ret_0_transfer := transfer_ERC20(this, msgsender_MSG, msgvalue_MSG, recipient_s267, amount_s267);
+}
 } else if ((choice) == (5)) {
 gas := (gas) - (21000);
+if ((gas) >= (0)) {
+assume ((msgvalue_MSG) == (0));
 call __ret_0_allowance := allowance_ERC20(this, msgsender_MSG, msgvalue_MSG, owner_s302, spender_s302);
+}
 } else if ((choice) == (4)) {
 gas := (gas) - (21000);
+if ((gas) >= (0)) {
+assume ((msgvalue_MSG) == (0));
 call __ret_0_approve := approve_ERC20(this, msgsender_MSG, msgvalue_MSG, spender_s317, amount_s317);
+}
 } else if ((choice) == (3)) {
 gas := (gas) - (21000);
+if ((gas) >= (0)) {
+assume ((msgvalue_MSG) == (0));
 call __ret_0_transferFrom := transferFrom_ERC20(this, msgsender_MSG, msgvalue_MSG, sender_s354, recipient_s354, amount_s354);
+}
 } else if ((choice) == (2)) {
 gas := (gas) - (21000);
+if ((gas) >= (0)) {
+assume ((msgvalue_MSG) == (0));
 call __ret_0_increaseAllowance := increaseAllowance_ERC20(this, msgsender_MSG, msgvalue_MSG, spender_s404, addedValue_s404);
+}
 } else if ((choice) == (1)) {
 gas := (gas) - (21000);
+if ((gas) >= (0)) {
+assume ((msgvalue_MSG) == (0));
 call __ret_0_decreaseAllowance := decreaseAllowance_ERC20(this, msgsender_MSG, msgvalue_MSG, spender_s446, subtractedValue_s446);
 }
 }
+}
 
-implementation CorralEntry_ERC20()
+implementation main()
 {
 var this: Ref;
 var msgsender_MSG: Ref;
 var msgvalue_MSG: int;
+assume ((null) == (0));
+call this := FreshRefGenerator__success();
+assume ((now) >= (0));
 assume ((DType[this]) == (ERC20));
 gas := (gas) - (53000);
 call ERC20_ERC20__success(this, msgsender_MSG, msgvalue_MSG);
